Add doc comments to chase definitions

ExistentialRules/ChaseSequence/TreeDerivation.lean
@@ -4,7 +4,34 @@ import ExistentialRules.Models.Basic
 import ExistentialRules.ChaseSequence.ChaseDerivation
 import ExistentialRules.ChaseSequence.ChaseNode
 
+/-!
+# Tree Derivation
+
+The `TreeDerivation` is the tree version of the `ChaseDerivation`.
+Since we allow rules to feature disjunctions,
+there are multiple possible results for a given trigger. The `ChaseDerivation` picks one possible choice.
+For the `TreeDerivation`, we consider all possiblities at once. That is, the tree branches out for the disjunctions.
+
+We try to mimic much of the machinery introduced for `ChaseDerivation` but we will see that some of this requires a different approach.
+Most prominently, we now need to consider addresses of nodes in the tree to be able to define a proper predecessor relation.
+-/
+
 variable {sig : Signature} [DecidableEq sig.P] [DecidableEq sig.C] [DecidableEq sig.V]
+
+section ChaseStep
+
+/-!
+## Chase Step
+
+To define how one chase step follows from the previous, we introduce two auxiliary definitions that capture two cases that can occur for a given `ChaseNode` in a `TreeDerivation`. This is similar to the definitions for `ChaseDerivation` only that now the result is a list of `ChaseNode`s.
+
+1. Case (`exists_trigger_list`): There still exists an `active` trigger,
+in which case one chase node for each disjunct of the trigger is introduced and contains
+the facts from the previous step together with the respective head result of the trigger.
+
+2. Case (`not_exists_trigger_list`): There is no active trigger.
+Then the successor list must be empty, i.e. the respective tree node does not have any children.
+-/
 
 def exists_trigger_list_condition (obs : ObsoletenessCondition sig) (rules : RuleSet sig) (before : ChaseNode obs rules) (after : List (ChaseNode obs rules)) (trg : RTrigger obs rules) : Prop :=
   trg.val.active before.facts ∧ after = trg.val.mapped_head.zipIdx_with_lt.attach.map (fun ⟨⟨head, i⟩, h⟩ => {
@@ -25,6 +52,21 @@ def exists_trigger_list (obs : ObsoletenessCondition sig) (rules : RuleSet sig) 
 def not_exists_trigger_list (obs : ObsoletenessCondition sig) (rules : RuleSet sig) (before : ChaseNode obs rules) (after : List (ChaseNode obs rules)) : Prop :=
   ¬(∃ trg : (RTrigger obs rules), trg.val.active before.facts) ∧ after = []
 
+end ChaseStep
+
+/-!
+## The TreeDerivation Structure
+
+The backbone of the `TreeDerivation` is a `FiniteDegreeTree` of `ChaseNode`s with a couple of conditions.
+
+1. We enforce that there is at least an initial `ChaseNode`.
+2. At each step in the derivation, either there exists a trigger that yields the child nodes or there is no trigger and consequently the derivation stops at this point. This is expressed by the two auxiliary definitions above.
+3. No triggers are active on leaf nodes.
+4. For each trigger, there exists a depth in the tree from which on the trigger is never active anymore.
+
+Conditions 3 and 4 together are "fairness", i.e. each trigger must eventually be non-active. Fairness ensures that the chase result (or in this case each fact set in the chase result) is indeed a model.
+-/
+
 structure TreeDerivation (obs : ObsoletenessCondition sig) (rules : RuleSet sig) where
   tree : FiniteDegreeTree (ChaseNode obs rules)
   isSome_root : tree.root.isSome
@@ -39,84 +81,590 @@ structure TreeDerivation (obs : ObsoletenessCondition sig) (rules : RuleSet sig)
 
 namespace TreeDerivation
 
-  variable {obs : ObsoletenessCondition sig} {rules : RuleSet sig}
+variable {obs : ObsoletenessCondition sig} {rules : RuleSet sig}
 
-  def toFiniteDegreeTreeWithRoot (td : TreeDerivation obs rules) : FiniteDegreeTree.FiniteDegreeTreeWithRoot (ChaseNode obs rules) :=
-    ⟨td.tree, by rw [← Option.isSome_iff_ne_none]; exact td.isSome_root⟩
+section Basics
 
-  instance : Membership (ChaseNode obs rules) (TreeDerivation obs rules) where
-    mem td node := node ∈ td.tree
+/-!
+## Basic Definitions
 
-  def derivation_for_branch (td : TreeDerivation obs rules) (branch : PossiblyInfiniteList (ChaseNode obs rules)) (branch_mem : branch ∈ td.tree.branches) : ChaseDerivation obs rules := {
-    branch := branch,
-    isSome_head := by
-      rw [FiniteDegreeTree.branches_eq] at branch_mem
-      rcases branch_mem with ⟨head_eq, _⟩
-      rw [head_eq]
-      exact td.isSome_root
-    triggers_exist := by
-      rcases branch_mem with ⟨ns, branch_eq, ns_max⟩
-      have branch_eq2 : ∀ n, (branch.drop n).head = (td.tree.drop (ns.take n)).root := by intro n; rw [branch_eq, FiniteDegreeTree.root_drop]; rfl
+Here we introduce some auxiliary definitions and theorems and we lift some of the machinery of the underlying `FiniteDegreeTree` to `TreeDerivation`.
+-/
 
-      intro n node node_mem
-      cases td.triggers_exist (ns.take n) node (by rw [← branch_eq2]; exact node_mem) with
-      | inl trg_ex =>
-        apply Or.inl
-        rcases trg_ex with ⟨trg, trg_ex⟩
-        exists trg
+/-- We can convert a `TreeDerivation` directly to a `FiniteDegreeTreeWithRoot`. -/
+def toFiniteDegreeTreeWithRoot (td : TreeDerivation obs rules) : FiniteDegreeTree.FiniteDegreeTreeWithRoot (ChaseNode obs rules) :=
+  ⟨td.tree, by rw [← Option.isSome_iff_ne_none]; exact td.isSome_root⟩
+
+/-- Membership of `ChaseNode`s in the `TreeDerivation` directly corresponds to membership in the `FiniteDegreeTree`. -/
+instance : Membership (ChaseNode obs rules) (TreeDerivation obs rules) where
+  mem td node := node ∈ td.tree
+
+/-- Each subtree of the underlying `FiniteDegreeTree` is itself a `TreeDerivation` as long as its root is not none. -/
+def derivation_for_suffix
+    (td : TreeDerivation obs rules)
+    (t2 : FiniteDegreeTree (ChaseNode obs rules))
+    (suffix : t2 <:+ td.tree)
+    (t2_root_some : t2.root.isSome) :
+    TreeDerivation obs rules where
+  tree := t2
+  isSome_root := t2_root_some
+  triggers_exist := by
+    rw [FiniteDegreeTree.IsSuffix_iff] at suffix
+    rcases suffix with ⟨ms, suffix⟩
+    rw [← suffix]
+    intro ns
+    have := td.triggers_exist (ms ++ ns)
+    simp only [FiniteDegreeTree.root_drop, FiniteDegreeTree.drop_drop] at *
+    exact this
+  fairness_leaves := by
+    rw [FiniteDegreeTree.IsSuffix_iff] at suffix
+    rcases suffix with ⟨ms, suffix⟩
+    intro leaf leaf_mem
+    rcases leaf_mem with ⟨ns, leaf_mem⟩
+    simp only [← suffix, FiniteDegreeTree.drop, PossiblyInfiniteTree.drop_drop] at leaf_mem
+    apply td.fairness_leaves
+    exists (ms ++ ns)
+  fairness_infinite_branches := by
+    rw [Option.isSome_iff_exists] at t2_root_some; rcases t2_root_some with ⟨t2_root, t2_root_eq⟩
+    rw [FiniteDegreeTree.IsSuffix_iff] at suffix
+    rcases suffix with ⟨ms, suffix⟩
+    rw [← suffix]
+    intro trg
+    rcases td.fairness_infinite_branches trg with ⟨i, fairness⟩
+    exists i
+    intro ns ns_length
+    rw [FiniteDegreeTree.get?_drop]
+    apply fairness (ms ++ ns)
+    rw [List.length_append, ge_iff_le]
+    apply Nat.le_add_left_of_le
+    exact ns_length
+
+/-- The root of the `TreeDerivation` is the initial `ChaseNode`. We know that this is never none. -/
+def root (td : TreeDerivation obs rules) : ChaseNode obs rules := td.tree.root.get (td.isSome_root)
+
+/-- The `root` is a member. -/
+theorem root_mem {td : TreeDerivation obs rules} : td.root ∈ td := by exists []; simp [root, FiniteDegreeTree.root_eq, FiniteDegreeTree.get?, PossiblyInfiniteTree.get?]
+
+section ChildNodes
+
+/-!
+### The (immediate) ChildNodes
+
+For a `TreeDerivation` derivation, its `childNodes` are the `ChaseNode`s immediately following the `root`.
+We mainly introduce a couple of theorems here that abstract away the `triggers_exist` condition from the `TreeDerivation` definition.
+-/
+
+def childNodes (td : TreeDerivation obs rules) : List (ChaseNode obs rules) := td.tree.childNodes
+
+/-- Each child node is a member. -/
+theorem mem_of_mem_childNodes {td : TreeDerivation obs rules} : ∀ n ∈ td.childNodes, n ∈ td := FiniteDegreeTree.mem_of_mem_childNodes
+
+/-- The origin of the `childNodes` needs to be set. -/
+theorem isSome_origin_of_mem_childNodes {td : TreeDerivation obs rules} : ∀ n ∈ td.childNodes, n.origin.isSome := by
+  intro n n_mem
+  have trg_ex := td.triggers_exist []
+  rw [FiniteDegreeTree.drop_nil] at trg_ex
+  specialize trg_ex td.root (by simp [root])
+  cases trg_ex with
+  | inl trg_ex => rcases trg_ex with ⟨_, _, trg_ex⟩; unfold childNodes at n_mem; rw [trg_ex] at n_mem; simp only [List.mem_map] at n_mem; rcases n_mem with ⟨a, _, eq⟩; rw [← eq]; simp
+  | inr trg_ex => have contra := trg_ex.right; unfold childNodes at n_mem; rw [contra] at n_mem; simp at n_mem
+
+/-- The trigger used to derive the `childNodes` is active for `head`. -/
+theorem active_trigger_origin_of_mem_childNodes {td : TreeDerivation obs rules} :
+    ∀ {n}, (mem : n ∈ td.childNodes) -> (n.origin.get (td.isSome_origin_of_mem_childNodes _ mem)).fst.val.active td.root.facts := by
+  intro n n_mem
+  have trg_ex := td.triggers_exist []
+  rw [FiniteDegreeTree.drop_nil] at trg_ex
+  specialize trg_ex td.root (by simp [root])
+  cases trg_ex with
+  | inl trg_ex => rcases trg_ex with ⟨_, trg_act, trg_ex⟩; unfold childNodes at n_mem; rw [trg_ex] at n_mem; simp only [List.mem_map] at n_mem; rcases n_mem with ⟨a, _, eq⟩; simp only [← eq]; exact trg_act
+  | inr trg_ex => have contra := trg_ex.right; unfold childNodes at n_mem; rw [contra] at n_mem; simp at n_mem
+
+/-- The `childNodes` are not nil if and only if some trigger is active on `root`. -/
+theorem childNodes_ne_nil_iff_trg_ex {td : TreeDerivation obs rules} : td.childNodes ≠ [] ↔ ∃ (trg : RTrigger obs rules), trg.val.active td.root.facts := by
+  constructor
+  . rw [List.ne_nil_iff_exists_cons]
+    rintro ⟨hd, tl, eq⟩
+    exists (hd.origin.get (td.isSome_origin_of_mem_childNodes _ (by simp [eq]))).fst
+    apply active_trigger_origin_of_mem_childNodes
+    simp [eq]
+  . rintro ⟨trg, active⟩
+    intro eq_nil
+    apply td.fairness_leaves td.root _ trg active
+    exists []
+    simp only [root, Option.some_get, FiniteDegreeTree.root, PossiblyInfiniteTree.root_eq, true_and]
+    simp only [childNodes, FiniteDegreeTree.childNodes, PossiblyInfiniteList.toList_of_finite_empty_iff] at eq_nil
+    simp only [PossiblyInfiniteTree.drop_nil]
+    rw [← PossiblyInfiniteList.empty_iff_head_none]
+    exact eq_nil
+
+/-- The fact set of each of the `childNodes` consists exactly of the facts from `root` and the result of the trigger that introduces the child node. -/
+theorem facts_childNodes {td : TreeDerivation obs rules} :
+    ∀ {n}, (mem : n ∈ td.childNodes) -> n.facts = td.root.facts ∪ (n.origin_result (td.isSome_origin_of_mem_childNodes _ mem)).toSet := by
+  intro n n_mem
+  have trg_ex := td.triggers_exist []
+  rw [FiniteDegreeTree.drop_nil] at trg_ex
+  specialize trg_ex td.root (by simp [root])
+  cases trg_ex with
+  | inl trg_ex =>
+    rcases trg_ex with ⟨trg, trg_act, trg_ex⟩; unfold childNodes at n_mem; rw [trg_ex] at n_mem; simp only [List.mem_map] at n_mem
+    rcases n_mem with ⟨head, _, eq⟩; simp only [← eq]
+    have head_mem := head.property
+    rw [List.mem_zipIdx_with_lt_iff_mem_zipIdx, List.mem_zipIdx_iff_getElem?, List.getElem?_eq_some_iff] at head_mem
+    rcases head_mem with ⟨_, head_mem⟩
+    simp only at head_mem
+    simp only [← head_mem]
+    rfl
+  | inr trg_ex => have contra := trg_ex.right; unfold childNodes at n_mem; rw [contra] at n_mem; simp at n_mem
+
+end ChildNodes
+
+section Suffixes
+
+/-!
+### TreeDerivation Subtrees
+
+We define a suffix/subtree relation on `TreeDerivation` simply as the subtree relation of the underlying `FiniteDegreeTree`.
+-/
+
+def IsSuffix (td1 td2 : TreeDerivation obs rules) : Prop := td1.tree <:+ td2.tree
+infixl:50 " <:+ " => IsSuffix
+
+theorem IsSuffix_iff {td1 td2 : TreeDerivation obs rules} : td1 <:+ td2 ↔ td1.tree <:+ td2.tree := by rfl
+
+/-- Members of our subtrees are also our members. -/
+theorem mem_of_mem_suffix {cd1 cd2 : TreeDerivation obs rules} (suffix : cd1 <:+ cd2) : ∀ node ∈ cd1, node ∈ cd2 := FiniteDegreeTree.mem_of_mem_suffix suffix
+
+end Suffixes
+
+section ChildTrees
+
+/-!
+### Child Trees
+
+We can drop the root of a `TreeDerivation` and obtain a (possibly empty) list of `childTrees`, which are again `TreeDerivation`s.
+-/
+
+/-- We obtain the child trees of the `FiniteDegreeTree` and convert each of them into a `TreeDerivation` using `derivation_for_suffix`. We know that all of those trees have non-none roots. -/
+def childTrees (td : TreeDerivation obs rules) : List (TreeDerivation obs rules) :=
+  td.tree.childTrees.attach.map (fun t =>
+    td.derivation_for_suffix t.val (by apply FiniteDegreeTree.IsSuffix_of_mem_childTrees; exact t.property) (by rw [Option.isSome_iff_ne_none]; exact t.val.property)
+  )
+
+/-- Membership in `childTrees` can be boiled down to membership in `FiniteDegreeTree.childTrees`. -/
+theorem mem_childTrees_iff {td : TreeDerivation obs rules} : ∀ c, c ∈ td.childTrees ↔ c.toFiniteDegreeTreeWithRoot ∈ td.tree.childTrees := by
+  intro c
+  unfold childTrees toFiniteDegreeTreeWithRoot derivation_for_suffix
+  simp only [List.mem_map, List.mem_attach, true_and]
+  constructor
+  . rintro ⟨d, eq⟩; rw [← eq]; exact d.property
+  . intro mem; exists ⟨c.toFiniteDegreeTreeWithRoot, mem⟩
+
+/-- `childNodes` can be expressed by mapping each `childTrees` to its root. -/
+theorem childNodes_eq {td : TreeDerivation obs rules} : td.childNodes = td.childTrees.map root := by
+  unfold childNodes childTrees
+  rw [FiniteDegreeTree.childNodes_eq]
+  apply List.ext_getElem
+  . simp
+  . intro i _ _; simp [derivation_for_suffix, root]
+
+/-- Each `childTrees` is a suffix. -/
+theorem IsSuffix_of_mem_childTrees {td : TreeDerivation obs rules} : ∀ td2 ∈ td.childTrees, td2 <:+ td := by intro td2 mem; apply FiniteDegreeTree.IsSuffix_of_mem_childTrees td2.toFiniteDegreeTreeWithRoot; rw [← mem_childTrees_iff]; exact mem
+
+/-- A derivation is a subtree of another if and only if both are the same or the first is a suffix of one of the second's child trees. -/
+theorem suffix_iff_eq_or_suffix_childTree {td1 td2 : TreeDerivation obs rules} : td1 <:+ td2 ↔ td1 = td2 ∨ ∃ td3 ∈ td2.childTrees, td1 <:+ td3 := by
+  constructor
+  . rw [IsSuffix_iff, FiniteDegreeTree.IsSuffix_iff]; rintro ⟨ns, suffix⟩
+    cases ns with
+    | nil => apply Or.inl; rw [TreeDerivation.mk.injEq]; rw [FiniteDegreeTree.drop_nil] at suffix; apply Eq.symm; exact suffix
+    | cons hd tl =>
+      apply Or.inr
+      cases eq : td2.childTrees[hd]? with
+      | none =>
+        have contra := td1.isSome_root
+        rw [Option.isSome_iff_ne_none] at contra
+        apply False.elim; apply contra
+        have suf : td1.tree <:+ td2.tree.drop [hd] := by
+          rw [FiniteDegreeTree.IsSuffix_iff]
+          exists tl
+        rw [← FiniteDegreeTree.empty_iff_root_none]
+        simp only [childTrees, List.getElem?_map, List.getElem?_attach, Option.map_eq_none_iff, Option.pmap_eq_none_iff] at eq
+        rw [FiniteDegreeTree.get?_childTrees, FiniteDegreeTree.FiniteDegreeTreeWithRoot.tree_to_opt_none_iff] at eq
+        rw [← FiniteDegreeTree.empty_iff_root_none] at eq
+        rw [eq] at suf
+        apply FiniteDegreeTree.empty_suffix_of_empty suf
+      | some c =>
+        rw [List.getElem?_eq_some_iff] at eq
+        rcases eq with ⟨_, eq⟩
+        exists c
         constructor
-        . exact trg_ex.left
-        . cases Decidable.em (ns.get n < trg.val.rule.head.length) with
-          | inl n_lt_head_length =>
-            have length_aux_1 : ns.get n < trg.val.mapped_head.length := by
-              rw [trg.val.length_mapped_head]
-              exact n_lt_head_length
-            exists ⟨ns.get n, length_aux_1⟩
-            specialize branch_eq2 n.succ
-            rw [PossiblyInfiniteList.head_eq, PossiblyInfiniteList.get?_drop] at branch_eq2
-            rw [PossiblyInfiniteList.head_eq, PossiblyInfiniteList.get?_tail, PossiblyInfiniteList.get?_drop, branch_eq2]
-            rw [InfiniteList.take_succ', ← FiniteDegreeTree.drop_drop]
-            rw [← FiniteDegreeTree.FiniteDegreeTreeWithRoot.opt_to_tree_after_tree_to_opt (t := ((td.tree.drop (ns.take n)).drop [ns.get n]))]
-            rw [← FiniteDegreeTree.get?_childTrees]
-            rw [← FiniteDegreeTree.get?_childNodes]
-            rw [trg_ex.right]
-            simp only
-            rw [List.getElem?_eq_getElem (by rw [List.length_map, List.length_attach, List.length_zipIdx_with_lt]; exact length_aux_1)]
-            rw [Option.some_inj]
-            rw [List.getElem_map, List.getElem_attach, ChaseNode.mk.injEq]
-            rw [List.zipIdx_with_lt_getElem_fst_eq_getElem]
-            rw [List.zipIdx_with_lt_getElem_snd_eq_index]
-            constructor
-            . rfl
-            . rfl
-          | inr n_lt_head_length =>
-            have : (td.tree.drop (ns.take n)).childNodes[ns.get n]? = none := by
-              rw [trg_ex.right]
-              apply List.getElem?_eq_none
-              apply Nat.le_of_not_lt
-              rw [List.length_map, List.length_attach, List.length_zipIdx_with_lt, trg.val.length_mapped_head]
-              exact n_lt_head_length
-            have : node ∈ td.tree.leaves := by
-              unfold FiniteDegreeTree.leaves
-              unfold PossiblyInfiniteTree.leaves
-              exists (ns.take n)
-              constructor
-              . rw [branch_eq2, FiniteDegreeTree.root_drop] at node_mem
-                exact node_mem
-              . apply ns_max
-                rw [PossiblyInfiniteTree.get?_branchForAddress, InfiniteList.take_succ']
-                rw [FiniteDegreeTree.get?_childNodes, ← FiniteDegreeTree.FiniteDegreeTreeWithRoot.opt_to_tree_none_iff] at this
-                rw [FiniteDegreeTree.get?_childTrees, FiniteDegreeTree.FiniteDegreeTreeWithRoot.tree_to_opt_none_iff] at this
-                rw [FiniteDegreeTree.drop_drop, FiniteDegreeTree.root_drop] at this
-                exact this
-            have not_active : ¬ trg.val.active node.facts := by apply td.fairness_leaves; exact this
-            have active : trg.val.active node.facts := trg_ex.left
-            contradiction
-      | inr trg_ex =>
-        apply Or.inr
-        constructor
-        . exact trg_ex.left
-        . specialize branch_eq2 n.succ
+        . simp [← eq]
+        . rw [IsSuffix_iff, FiniteDegreeTree.IsSuffix_iff]; exists tl; rw [← eq]; simp only [childTrees, derivation_for_suffix, List.getElem_map, List.getElem_attach, FiniteDegreeTree.get_childTrees]; exact suffix
+  . intro h; cases h with
+    | inl eq => rw [eq]; exact FiniteDegreeTree.IsSuffix_refl
+    | inr suffix => rcases suffix with ⟨td3, td3_mem, suffix⟩; apply FiniteDegreeTree.IsSuffix_trans suffix; exact IsSuffix_of_mem_childTrees _ td3_mem
+
+end ChildTrees
+
+section InductionPrinciple
+
+/-!
+### Induction Principle for Members
+
+Similar to `FiniteDegreeTree.mem_rec`, we define an induction principle to show
+properties of `ChaseNode`s in a `TreeDerivation`.
+
+Looking ahead a bit, we will also want to define a predecessor relation on nodes in the tree as we did for nodes in a `ChaseDerivation`.
+This is not so elegant here though as the same node might indeed occur multiple times in the tree.
+Therefore, we are going to associate each node with its address in the tree to tell them apart.
+Since we are doing this anyway, it makes sense to define the induction principle already with respect to this kind of node.
+-/
+
+/-!
+#### NodeWithAddress
+
+The `NodeWithAddress` is a structure of a `ChaseNode`, an address (i.e. a `List Nat`), and a proof that the chase node is indeed at the given address.
+We also introduce a couple of covenience functions and theorems for the `NodeWithAddress`.
+-/
+
+structure NodeWithAddress (td : TreeDerivation obs rules) where
+  node : ChaseNode obs rules
+  address : List Nat
+  eq : td.tree.get? address = some node
+
+namespace NodeWithAddress
+
+/-- Each `NodeWithAddress` induces a `subderivation` in the `TreeDerivation`. -/
+def subderivation {td : TreeDerivation obs rules} (node : NodeWithAddress td) : TreeDerivation obs rules :=
+  td.derivation_for_suffix (td.tree.drop node.address) (td.tree.IsSuffix_drop node.address) (by simp [FiniteDegreeTree.root_drop, node.eq])
+
+/-- We can cast a node for one of our subderivations into our own node. -/
+def cast_for_new_root_node
+    {td : TreeDerivation obs rules}
+    (new_root : NodeWithAddress td)
+    (node : new_root.subderivation.NodeWithAddress) :
+    NodeWithAddress td where
+  node := node.node
+  address := new_root.address ++ node.address
+  eq := by
+    rw [← node.eq]
+    simp only [subderivation, derivation_for_suffix, FiniteDegreeTree.get?_drop]
+
+/-- The `NodeWithAddress` version of `TreeDerivation.root`. -/
+def root (td : TreeDerivation obs rules) : NodeWithAddress td where
+  node := td.root
+  address := []
+  eq := by simp [TreeDerivation.root, FiniteDegreeTree.root_eq]
+
+/-- The `NodeWithAddress` version of `TreeDerivation.childNodes`. -/
+def childNodes (td : TreeDerivation obs rules) : List (NodeWithAddress td) := td.childNodes.zipIdx_with_lt.attach.map (fun ⟨⟨c, idx⟩, prop⟩ => {
+  node := c
+  address := [idx.val]
+  eq := by
+    rw [List.mem_zipIdx_with_lt_iff_mem_zipIdx, List.mem_zipIdx_iff_getElem?] at prop
+    simp only [TreeDerivation.childNodes, FiniteDegreeTree.get?_childNodes, FiniteDegreeTree.get?_childTrees, FiniteDegreeTree.FiniteDegreeTreeWithRoot.opt_to_tree_after_tree_to_opt] at prop
+    exact prop
+})
+
+/-- The `NodeWithAddress` is a member. -/
+theorem mem {td : TreeDerivation obs rules} (node : td.NodeWithAddress) : node.node ∈ td := by exists node.address; exact node.eq
+
+/-- Two `NodeWithAddress` are equal if their addresses are. -/
+theorem eq_of_address_eq {td : TreeDerivation obs rules} {n1 n2 : td.NodeWithAddress} : n1.address = n2.address -> n1 = n2 := by
+  intro eq
+  rw [NodeWithAddress.mk.injEq]
+  simp only [eq, and_true]
+  have eq1 := n1.eq
+  have eq2 := n2.eq
+  rw [eq] at eq1
+  rw [eq1, Option.some_inj] at eq2
+  exact eq2
+
+/-- `subderivation` is indeed a subtree. -/
+theorem IsSuffix_subderivation {td : TreeDerivation obs rules} {node : NodeWithAddress td} : node.subderivation <:+ td := td.tree.IsSuffix_drop node.address
+
+/-- The root of the `subderivation` is the node itself with empty address. -/
+theorem root_subderivation {td : TreeDerivation obs rules} {node : NodeWithAddress td} : (root node.subderivation) = { node := node.node, address := [], eq := by simp only [subderivation, derivation_for_suffix, FiniteDegreeTree.get?_drop, List.append_nil]; exact node.eq } := by
+  simp [subderivation, derivation_for_suffix, root, TreeDerivation.root, FiniteDegreeTree.root_drop, node.eq]
+
+/-- The root of the `subderivation` is the node itself. -/
+theorem root_subderivation' {td : TreeDerivation obs rules} {node : NodeWithAddress td}: node.subderivation.root = node.node := by
+  simp [subderivation, derivation_for_suffix, TreeDerivation.root, FiniteDegreeTree.root_drop, node.eq]
+
+/-- `NodeWithAddress.childNodes` has the same length as `TreeDerivation.childNodes`. -/
+theorem length_childNodes {td : TreeDerivation obs rules} : (childNodes td).length = td.childNodes.length := by
+  simp [childNodes, List.length_zipIdx_with_lt]
+
+/-- `NodeWithAddress.childNodes` and `TreeDerivation.childNodes` are (almost) equal. -/
+theorem childNodes_eq_childNodes {td : TreeDerivation obs rules} : td.childNodes = (childNodes td).map NodeWithAddress.node := by
+  apply List.ext_getElem
+  . rw [List.length_map, length_childNodes]
+  intro i _ _
+  simp only [childNodes, List.getElem_map, List.getElem_attach]
+  rw [List.zipIdx_with_lt_getElem_fst_eq_getElem]
+
+/-- Membership for `NodeWithAddress.childNodes` and `TreeDerivation.childNodes` is (almost) the same. -/
+theorem mem_childNodes_of_mem_childNodes {td : TreeDerivation obs rules} : ∀ {n}, n ∈ (childNodes td) -> n.node ∈ td.childNodes := by
+  intro n n_mem; rw [childNodes_eq_childNodes]; apply List.mem_map_of_mem; exact n_mem
+
+/-- Getting specific elements from child nodes can be translated between `NodeWithAddress.childNodes` and `TreeDerivation.childNodes`. -/
+theorem node_getElem_childNodes {td : TreeDerivation obs rules} : ∀ i (lt : i < (childNodes td).length), (childNodes td)[i].node = td.childNodes[i]'(by rw [← length_childNodes]; exact lt) := by simp [childNodes_eq_childNodes]
+
+/-- The subderivation for a child node is a child tree. -/
+theorem subderivation_mem_childTrees_of_mem_childNodes {td : TreeDerivation obs rules} {node : NodeWithAddress td} :
+    node ∈ (childNodes td) -> node.subderivation ∈ td.childTrees := by
+  intro node_mem
+  simp only [childNodes, List.mem_map, List.mem_attach, true_and] at node_mem
+  rcases node_mem with ⟨⟨node_with_idx, node_mem⟩, node_eq⟩
+  rw [List.mem_zipIdx_with_lt_iff_mem_zipIdx] at node_mem
+  have node_mem := List.mem_zipIdx' node_mem
+  have : node.subderivation = td.childTrees[node_with_idx.snd.val]'(by have lt := node_with_idx.snd.isLt; simp only [childNodes_eq, List.length_map] at lt; exact lt) := by
+    simp only [childTrees, List.getElem_map, List.getElem_attach, FiniteDegreeTree.get_childTrees]
+    simp only [subderivation]
+    rw [← node_eq]
+  rw [this]
+  apply List.getElem_mem
+
+end NodeWithAddress
+
+/-!
+Now we are ready for the actual induction principle on `NodeWithAddress`s in a `TreeDerivation`.
+-/
+
+/-- If we want to show a motive for all nodes in a derivation, it is enough to show the motive for the root and for each arbitrary child node in each abitrary subderivation where the motive in turn already holds for the root. This can be used with the induction tactic. -/
+theorem mem_rec_address
+    {td : TreeDerivation obs rules}
+    {motive : NodeWithAddress td -> Prop}
+    (root : motive (NodeWithAddress.root td))
+    (step : ∀ (new_root : NodeWithAddress td), motive new_root -> ∀ c, (mem : c ∈ (NodeWithAddress.childNodes new_root.subderivation)) -> motive (NodeWithAddress.cast_for_new_root_node new_root c))
+    (node : NodeWithAddress td) :
+    motive node := by
+  let motive' (rev_addr : List Nat) := ∀ n, (mem : n ∈ td.tree.get? rev_addr.reverse) -> motive {
+    node := n
+    address := rev_addr.reverse
+    eq := mem
+  }
+  let rev_addr_node := node.address.reverse
+  have : motive' rev_addr_node := by
+    induction rev_addr_node with
+    | nil =>
+      intro n n_mem
+      have eq : NodeWithAddress.root td = {node := n, address := [].reverse, eq := n_mem} := by
+        apply NodeWithAddress.eq_of_address_eq; simp [NodeWithAddress.root]
+      rw [← eq]
+      exact root
+    | cons hd tl ih =>
+      intro n n_mem
+      cases eq : td.tree.get? tl.reverse with
+      | none =>
+        have contra := td.tree.no_orphans (td.tree.drop tl.reverse) (FiniteDegreeTree.IsSuffix_drop tl.reverse) (by rw [FiniteDegreeTree.root_drop]; exact eq)
+        have n_mem : n ∈ (td.tree.drop tl.reverse).childNodes[hd]? := by
+          rw [FiniteDegreeTree.get?_childNodes, FiniteDegreeTree.get?_childTrees, FiniteDegreeTree.FiniteDegreeTreeWithRoot.opt_to_tree_after_tree_to_opt]
+          rw [FiniteDegreeTree.drop_drop, FiniteDegreeTree.root_drop]
+          rw [List.reverse_cons] at n_mem
+          exact n_mem
+        simp [contra] at n_mem
+      | some m =>
+        have n_mem : n ∈ (td.tree.drop tl.reverse).childNodes[hd]? := by rw [FiniteDegreeTree.get?_childNodes, FiniteDegreeTree.get?_childTrees, FiniteDegreeTree.FiniteDegreeTreeWithRoot.opt_to_tree_after_tree_to_opt, FiniteDegreeTree.root_drop, FiniteDegreeTree.get?_drop]; rw [List.reverse_cons] at n_mem; exact n_mem
+        let new_root : td.NodeWithAddress := { node := m, address := tl.reverse, eq := eq }
+        specialize step new_root (ih m eq) _ (by
+          simp only [NodeWithAddress.childNodes, List.mem_map]
+          exists ⟨⟨n, ⟨hd, by
+              simp only [NodeWithAddress.subderivation, derivation_for_suffix, childNodes, new_root]
+              rw [Option.mem_def, List.getElem?_eq_some_iff] at n_mem
+              rcases n_mem with ⟨lt, _⟩
+              exact lt⟩⟩, by
+            rw [List.mem_zipIdx_with_lt_iff_mem_zipIdx, List.mem_zipIdx_iff_getElem?]
+            simp only [NodeWithAddress.subderivation, derivation_for_suffix, childNodes, new_root]
+            exact n_mem⟩
+          constructor; simp; rfl)
+        simp only [NodeWithAddress.cast_for_new_root_node, new_root] at step
+        simp only [List.reverse_cons]
+        exact step
+  specialize this node.node (by simp only [rev_addr_node, List.reverse_reverse]; exact node.eq)
+  simp only [rev_addr_node, List.reverse_reverse] at this
+  exact this
+
+/-- A node is a member of some element of `childTrees` if and only if there is a subderivation where the node occurs in the `childNodes`. Part of this proof uses the induction principle defined above. -/
+theorem mem_some_childTree_iff {td : TreeDerivation obs rules} {node : ChaseNode obs rules} :
+    (∃ t ∈ td.childTrees, node ∈ t) ↔ ∃ td2, td2 <:+ td ∧ node ∈ td2.childNodes := by
+  constructor
+  . rintro ⟨t, t_mem, node_mem⟩
+    rcases node_mem with ⟨addr, node_mem⟩
+    let node' : t.NodeWithAddress := { node := node, address := addr, eq := node_mem }
+    show ∃ td2, td2 <:+ td ∧ node'.node ∈ td2.childNodes
+    induction node' using mem_rec_address with
+    | root => exists td; constructor; exact td.tree.IsSuffix_refl; simp only [childNodes_eq, NodeWithAddress.root]; apply List.mem_map_of_mem; exact t_mem
+    | step new_root ih c c_mem =>
+      exists new_root.subderivation; constructor
+      . apply FiniteDegreeTree.IsSuffix_trans NodeWithAddress.IsSuffix_subderivation; exact IsSuffix_of_mem_childTrees _ t_mem
+      . rw [NodeWithAddress.childNodes_eq_childNodes]; apply List.mem_map_of_mem; exact c_mem
+  . rintro ⟨td2, suffix, node_mem⟩
+    rw [IsSuffix_iff, FiniteDegreeTree.IsSuffix_iff] at suffix; rcases suffix with ⟨ns, suffix⟩
+    cases ns with
+    | nil =>
+      have : td = td2 := by rw [TreeDerivation.mk.injEq]; rw [FiniteDegreeTree.drop_nil] at suffix; exact suffix
+      rw [childNodes_eq, List.mem_map] at node_mem; rcases node_mem with ⟨t, t_mem, node_mem⟩; exists t; constructor; rw [this]; exact t_mem; rw [← node_mem]; exact root_mem
+    | cons hd tl =>
+      cases eq : td.childTrees[hd]? with
+      | none =>
+        have contra := td2.isSome_root
+        rw [Option.isSome_iff_ne_none] at contra
+        apply False.elim; apply contra
+        have suf : td2.tree <:+ td.tree.drop [hd] := by
+          rw [FiniteDegreeTree.IsSuffix_iff]
+          exists tl
+        rw [← FiniteDegreeTree.empty_iff_root_none]
+        simp only [childTrees, List.getElem?_map, List.getElem?_attach, Option.map_eq_none_iff, Option.pmap_eq_none_iff] at eq
+        rw [FiniteDegreeTree.get?_childTrees, FiniteDegreeTree.FiniteDegreeTreeWithRoot.tree_to_opt_none_iff] at eq
+        rw [← FiniteDegreeTree.empty_iff_root_none] at eq
+        rw [eq] at suf
+        apply FiniteDegreeTree.empty_suffix_of_empty suf
+      | some t =>
+        rw [List.getElem?_eq_some_iff] at eq; rcases eq with ⟨_, eq⟩
+        exists t; constructor; simp [← eq]
+        have : td2 <:+ t := by rw [IsSuffix_iff, FiniteDegreeTree.IsSuffix_iff]; exists tl; rw [← eq]; simp only [childTrees, derivation_for_suffix, List.getElem_map, List.getElem_attach, FiniteDegreeTree.get_childTrees]; rw [FiniteDegreeTree.drop_drop, List.singleton_append]; exact suffix
+        apply mem_of_mem_suffix this
+        apply mem_of_mem_childNodes
+        exact node_mem
+
+end InductionPrinciple
+
+end Basics
+
+section FactMonotonicity
+
+/-!
+## Subset Monotonicity of Facts in ChaseNodes
+
+Since `ChaseNodes` always extend the previous facts, the fact sets can only be growing along the branches of the `TreeDerivation`.
+This has a couple of convenient implications. For example, the root of a `TreeDerivation` can never occur in its `childTrees`.
+-/
+
+/-- Each member's facts contain the root facts. -/
+theorem facts_node_subset_every_mem {td : TreeDerivation obs rules} : ∀ node ∈ td, td.root.facts ⊆ node.facts := by
+  rintro node ⟨addr, node_mem⟩
+  let node' : td.NodeWithAddress := { node := node, address := addr, eq := node_mem }
+  show td.root.facts ⊆ node'.node.facts
+  induction node' using mem_rec_address with
+  | root => apply Set.subset_refl
+  | step new_root ih c c_mem =>
+    apply Set.subset_trans ih
+    simp only [NodeWithAddress.cast_for_new_root_node]
+    rw [facts_childNodes (NodeWithAddress.mem_childNodes_of_mem_childNodes c_mem)]
+    apply Set.subset_union_of_subset_left
+    rw [NodeWithAddress.root_subderivation']
+    apply Set.subset_refl
+
+/-- The `root` cannot occur in the `childTrees`. Otherwise, it would be introduced using a trigger but then this trigger is already obsolete since all the facts from `root` already occur in the very beginning. We use `ObsoletenessCondition.contains_trg_result_implies_cond` here. -/
+theorem root_not_mem_childTrees {td : TreeDerivation obs rules} : ¬ ∃ t ∈ td.childTrees, td.root ∈ t := by
+  intro contra
+  rw [mem_some_childTree_iff] at contra
+  rcases contra with ⟨td2, suffix, contra⟩
+  apply (td2.active_trigger_origin_of_mem_childNodes contra).right
+  apply obs.contains_trg_result_implies_cond
+  apply Set.subset_trans (td.root.facts_contain_origin_result (td.root.origin.get (td2.isSome_origin_of_mem_childNodes _ contra)) (by simp))
+  apply td.facts_node_subset_every_mem
+  apply mem_of_mem_suffix suffix
+  exact td2.root_mem
+
+/-- By `root_not_mem_childTrees`, if we have a subtree but our root occurs in the subtree, then our subtree is equal to us. -/
+theorem eq_of_suffix_of_root_mem {td1 td2 : TreeDerivation obs rules} (suffix : td1 <:+ td2) (root_mem : td2.root ∈ td1) : td1 = td2 := by
+  rw [suffix_iff_eq_or_suffix_childTree] at suffix
+  cases suffix with
+  | inl suffix => exact suffix
+  | inr suffix => rcases suffix with ⟨td3, td3_mem, suffix⟩; apply False.elim; apply td2.root_not_mem_childTrees; exists td3; constructor; exact td3_mem; apply mem_of_mem_suffix suffix; exact root_mem
+
+end FactMonotonicity
+
+section Predecessors
+
+/-!
+## Predecessor Relation
+
+Opposed to the `ChaseDerivation`, we define the predecessor relation direclty using addresses here.
+This is because `ChaseNode`s may indeed occur multiple times in a `TreeDerivation` (just not in the same branch)
+and therefore the approach used in `ChaseDerivation` would not quite work.
+In particular, note that the `TreeDerivation` has no equivalent for `ChaseDerivation.suffix_of_suffix_of_suffix_of_head_mem`.
+
+Also, even with the address approach, the relation is not total here (which is expected for a tree).
+-/
+
+/-- Node $n$ is a predecessor of node $m$ if the address of $n$ is a prefix of the address of $m$. Predecessor can therefore also be understood as ancestor in the tree. -/
+def predecessor {td : TreeDerivation obs rules} (n1 n2 : NodeWithAddress td) : Prop := n1.address <+: n2.address
+infixl:50 " ≼ " => predecessor
+
+/-- The predecessor relation is stable across suffixes. That is, predecessor in our suffix are also predecessor for us. We only need to cast the nodes. -/
+theorem predecessor_of_suffix {td : TreeDerivation obs rules} {new_root : NodeWithAddress td} {n1 n2 : NodeWithAddress new_root.subderivation} : n1 ≼ n2 -> (new_root.cast_for_new_root_node n1) ≼ (new_root.cast_for_new_root_node n2) := by
+  rintro ⟨addr, eq⟩
+  exists addr
+  simp only [NodeWithAddress.cast_for_new_root_node]
+  simp [← eq]
+
+/-- The predecessor relation is reflexive. -/
+theorem predecessor_refl {td : TreeDerivation obs rules} {node : NodeWithAddress td} : node ≼ node := List.prefix_rfl
+
+/-- The predecessor relation is antisymmetric. -/
+theorem predecessor_antisymm {td : TreeDerivation obs rules} {n1 n2 : NodeWithAddress td} : n1 ≼ n2 -> n2 ≼ n1 -> n1 = n2 := by
+  rintro prefix1 ⟨addr2, prefix2⟩
+  apply NodeWithAddress.eq_of_address_eq
+  apply List.IsPrefix.eq_of_length_le prefix1
+  simp [← prefix2]
+
+/-- The predecessor relation is transitive. -/
+theorem predecessor_trans {td : TreeDerivation obs rules} {n1 n2 n3 : NodeWithAddress td} : n1 ≼ n2 -> n2 ≼ n3 -> n1 ≼ n3 := List.IsPrefix.trans
+
+/-- The `root` is a predecessor of each `childNodes`. -/
+theorem root_prec_childNodes {td : TreeDerivation obs rules} : ∀ n ∈ NodeWithAddress.childNodes td, NodeWithAddress.root td ≼ n := by
+  intros; exact List.nil_prefix
+
+/-- The facts of our predecessor are a subset of our facts. -/
+theorem facts_node_subset_of_prec {td : TreeDerivation obs rules} {node1 node2 : td.NodeWithAddress} : node1 ≼ node2 -> node1.node.facts ⊆ node2.node.facts := by
+  rintro ⟨diff, addr_eq⟩
+  have := node1.subderivation.facts_node_subset_every_mem node2.node
+  rw [NodeWithAddress.root_subderivation'] at this
+  apply this
+  exists diff
+  rw [← node2.eq, ← addr_eq]
+  rfl
+
+end Predecessors
+
+section BranchesAndResult
+
+/-!
+## Branches and Chase Result
+
+Here, we define the result of a `TreeDerivation`, which requires us to also define the branches of the `TreeDerivation`. It should be no surprise that these are `ChaseDerivation`s. The result is then just the set of the results of all the `ChaseDerivation`s in the tree. We already know from the `ChaseDerivation` that each element of `TreeDerivation.result` is therefore a model of the rules.
+-/
+
+/-- Each branch of the underlying tree can be transformed into a proper `ChaseDerivation`. -/
+def derivation_for_branch (td : TreeDerivation obs rules) (branch : PossiblyInfiniteList (ChaseNode obs rules)) (branch_mem : branch ∈ td.tree.branches) : ChaseDerivation obs rules := {
+  branch := branch,
+  isSome_head := by
+    rw [FiniteDegreeTree.branches_eq] at branch_mem
+    rcases branch_mem with ⟨head_eq, _⟩
+    rw [head_eq]
+    exact td.isSome_root
+  triggers_exist := by
+    rcases branch_mem with ⟨ns, branch_eq, ns_max⟩
+    have branch_eq2 : ∀ n, (branch.drop n).head = (td.tree.drop (ns.take n)).root := by intro n; rw [branch_eq, FiniteDegreeTree.root_drop]; rfl
+
+    intro n node node_mem
+    cases td.triggers_exist (ns.take n) node (by rw [← branch_eq2]; exact node_mem) with
+    | inl trg_ex =>
+      apply Or.inl
+      rcases trg_ex with ⟨trg, trg_ex⟩
+      exists trg
+      constructor
+      . exact trg_ex.left
+      . cases Decidable.em (ns.get n < trg.val.rule.head.length) with
+        | inl n_lt_head_length =>
+          have length_aux_1 : ns.get n < trg.val.mapped_head.length := by
+            rw [trg.val.length_mapped_head]
+            exact n_lt_head_length
+          exists ⟨ns.get n, length_aux_1⟩
+          specialize branch_eq2 n.succ
           rw [PossiblyInfiniteList.head_eq, PossiblyInfiniteList.get?_drop] at branch_eq2
           rw [PossiblyInfiniteList.head_eq, PossiblyInfiniteList.get?_tail, PossiblyInfiniteList.get?_drop, branch_eq2]
           rw [InfiniteList.take_succ', ← FiniteDegreeTree.drop_drop]
@@ -124,650 +672,324 @@ namespace TreeDerivation
           rw [← FiniteDegreeTree.get?_childTrees]
           rw [← FiniteDegreeTree.get?_childNodes]
           rw [trg_ex.right]
-          simp
-    fairness := by
-      rcases branch_mem with ⟨ns, branch_eq, ns_max⟩
-      have branch_eq2 : ∀ n, (branch.drop n).head = (td.tree.drop (ns.take n)).root := by intro n; rw [branch_eq, FiniteDegreeTree.root_drop]; rfl
-
-      intro trg
-      -- Case Distinction: Is branch finite?
-      cases Classical.em (∃ n : Nat, td.tree.get? (ns.take n) ≠ none ∧ ∀ m : Nat, m > n -> td.tree.get? (ns.take m) = none) with
-      | inl h =>
-        rcases h with ⟨n, h⟩
-        exists n
-        constructor
-        . rcases Option.ne_none_iff_exists'.mp h.left with ⟨node, node_eq⟩
-          exists node
+          simp only
+          rw [List.getElem?_eq_getElem (by rw [List.length_map, List.length_attach, List.length_zipIdx_with_lt]; exact length_aux_1)]
+          rw [Option.some_inj]
+          rw [List.getElem_map, List.getElem_attach, ChaseNode.mk.injEq]
+          rw [List.zipIdx_with_lt_getElem_fst_eq_getElem]
+          rw [List.zipIdx_with_lt_getElem_snd_eq_index]
           constructor
-          . rw [branch_eq2, FiniteDegreeTree.root_drop]; exact node_eq
-          . apply td.fairness_leaves
-            exists ns.take n
+          . rfl
+          . rfl
+        | inr n_lt_head_length =>
+          have : (td.tree.drop (ns.take n)).childNodes[ns.get n]? = none := by
+            rw [trg_ex.right]
+            apply List.getElem?_eq_none
+            apply Nat.le_of_not_lt
+            rw [List.length_map, List.length_attach, List.length_zipIdx_with_lt, trg.val.length_mapped_head]
+            exact n_lt_head_length
+          have : node ∈ td.tree.leaves := by
+            unfold FiniteDegreeTree.leaves
+            unfold PossiblyInfiniteTree.leaves
+            exists (ns.take n)
             constructor
-            . exact node_eq
+            . rw [branch_eq2, FiniteDegreeTree.root_drop] at node_mem
+              exact node_mem
             . apply ns_max
-              apply h.right
-              simp
-        . intro m
-          rw [PossiblyInfiniteList.tail_drop, PossiblyInfiniteList.get?_drop, ← PossiblyInfiniteList.head_drop]
-          rw [branch_eq2]
-          rw [FiniteDegreeTree.root_drop]
-          rw [h.right _ (by omega)]
-          simp
-      | inr h =>
-        have h : ∀ n, td.tree.get? (ns.take n) ≠ none := by
-          intro n contra
-          induction n with
-          | zero => rw [InfiniteList.take_zero] at contra; rw [← FiniteDegreeTree.root_eq] at contra; have contra' := td.isSome_root; simp [contra] at contra'
-          | succ n ih =>
-            apply h
-            exists n
-            constructor
-            . exact ih
-            . intro m m_gt
-              rw [← FiniteDegreeTree.root_drop] at contra
-              simp only [FiniteDegreeTree.root] at contra
-              rw [← PossiblyInfiniteTree.empty_iff_root_none] at contra
-              rw [gt_iff_lt, ← Nat.succ_le_iff] at m_gt
-              rcases Nat.exists_eq_add_of_le m_gt with ⟨K, m_gt⟩
-              rw [m_gt, InfiniteList.take_add, ← FiniteDegreeTree.get?_drop]
-              simp only [FiniteDegreeTree.get?]
-              rw [contra, PossiblyInfiniteTree.get?_empty]
-        rcases td.fairness_infinite_branches trg with ⟨i, fairness⟩
-        exists i
+              rw [PossiblyInfiniteTree.get?_branchForAddress, InfiniteList.take_succ']
+              rw [FiniteDegreeTree.get?_childNodes, ← FiniteDegreeTree.FiniteDegreeTreeWithRoot.opt_to_tree_none_iff] at this
+              rw [FiniteDegreeTree.get?_childTrees, FiniteDegreeTree.FiniteDegreeTreeWithRoot.tree_to_opt_none_iff] at this
+              rw [FiniteDegreeTree.drop_drop, FiniteDegreeTree.root_drop] at this
+              exact this
+          have not_active : ¬ trg.val.active node.facts := by apply td.fairness_leaves; exact this
+          have active : trg.val.active node.facts := trg_ex.left
+          contradiction
+    | inr trg_ex =>
+      apply Or.inr
+      constructor
+      . exact trg_ex.left
+      . specialize branch_eq2 n.succ
+        rw [PossiblyInfiniteList.head_eq, PossiblyInfiniteList.get?_drop] at branch_eq2
+        rw [PossiblyInfiniteList.head_eq, PossiblyInfiniteList.get?_tail, PossiblyInfiniteList.get?_drop, branch_eq2]
+        rw [InfiniteList.take_succ', ← FiniteDegreeTree.drop_drop]
+        rw [← FiniteDegreeTree.FiniteDegreeTreeWithRoot.opt_to_tree_after_tree_to_opt (t := ((td.tree.drop (ns.take n)).drop [ns.get n]))]
+        rw [← FiniteDegreeTree.get?_childTrees]
+        rw [← FiniteDegreeTree.get?_childNodes]
+        rw [trg_ex.right]
+        simp
+  fairness := by
+    rcases branch_mem with ⟨ns, branch_eq, ns_max⟩
+    have branch_eq2 : ∀ n, (branch.drop n).head = (td.tree.drop (ns.take n)).root := by intro n; rw [branch_eq, FiniteDegreeTree.root_drop]; rfl
+
+    intro trg
+    -- Case Distinction: Is branch finite?
+    cases Classical.em (∃ n : Nat, td.tree.get? (ns.take n) ≠ none ∧ ∀ m : Nat, m > n -> td.tree.get? (ns.take m) = none) with
+    | inl h =>
+      rcases h with ⟨n, h⟩
+      exists n
+      constructor
+      . rcases Option.ne_none_iff_exists'.mp h.left with ⟨node, node_eq⟩
+        exists node
         constructor
-        . rcases Option.ne_none_iff_exists'.mp (h i) with ⟨node, node_eq⟩
-          rw [branch_eq2]
-          exists node
+        . rw [branch_eq2, FiniteDegreeTree.root_drop]; exact node_eq
+        . apply td.fairness_leaves
+          exists ns.take n
           constructor
-          . rw [FiniteDegreeTree.root_drop]
-            exact node_eq
-          . specialize fairness (ns.take i) (by rw [InfiniteList.length_take]; simp)
-            apply fairness
-            exact node_eq
-        . intro m
-          rw [PossiblyInfiniteList.tail_drop, PossiblyInfiniteList.get?_drop, ← PossiblyInfiniteList.head_drop]
-          rw [branch_eq2]
-          rw [FiniteDegreeTree.root_drop]
-          apply fairness
-          rw [InfiniteList.length_take]
-          omega
-  }
-
-  def branches (td : TreeDerivation obs rules) : Set (ChaseDerivation obs rules) := fun branch =>
-    branch.branch ∈ td.tree.branches
-
-  theorem derivation_for_branch_mem_branches {td : TreeDerivation obs rules} {branch : PossiblyInfiniteList (ChaseNode obs rules)} {branch_mem : branch ∈ td.tree.branches} :
-    td.derivation_for_branch branch branch_mem ∈ td.branches := branch_mem
-
-  def result (td : TreeDerivation obs rules) : Set (FactSet sig) := fun fs => ∃ branch, branch ∈ td.branches ∧ branch.result = fs
-
-  -- inspired by List.IsSuffix; see https://github.com/leanprover/lean4/blob/9d4ad1273f6cea397c3066c2c83062a4410d16bf/src/Init/Data/List/Basic.lean#L1205
-  def IsSuffix (td1 td2 : TreeDerivation obs rules) : Prop := td1.tree <:+ td2.tree
-  infixl:50 " <:+ " => IsSuffix
-
-  theorem IsSuffix_iff {td1 td2 : TreeDerivation obs rules} : td1 <:+ td2 ↔ td1.tree <:+ td2.tree := by rfl
-
-  theorem mem_of_mem_suffix {cd1 cd2 : TreeDerivation obs rules} (suffix : cd1 <:+ cd2) : ∀ node ∈ cd1, node ∈ cd2 := FiniteDegreeTree.mem_of_mem_suffix suffix
-
-  def derivation_for_suffix
-      (td : TreeDerivation obs rules)
-      (t2 : FiniteDegreeTree (ChaseNode obs rules))
-      (suffix : t2 <:+ td.tree)
-      (t2_root_some : t2.root.isSome) :
-      TreeDerivation obs rules where
-    tree := t2
-    isSome_root := t2_root_some
-    triggers_exist := by
-      rw [FiniteDegreeTree.IsSuffix_iff] at suffix
-      rcases suffix with ⟨ms, suffix⟩
-      rw [← suffix]
-      intro ns
-      have := td.triggers_exist (ms ++ ns)
-      simp only [FiniteDegreeTree.root_drop, FiniteDegreeTree.drop_drop] at *
-      exact this
-    fairness_leaves := by
-      rw [FiniteDegreeTree.IsSuffix_iff] at suffix
-      rcases suffix with ⟨ms, suffix⟩
-      intro leaf leaf_mem
-      rcases leaf_mem with ⟨ns, leaf_mem⟩
-      simp only [← suffix, FiniteDegreeTree.drop, PossiblyInfiniteTree.drop_drop] at leaf_mem
-      apply td.fairness_leaves
-      exists (ms ++ ns)
-    fairness_infinite_branches := by
-      rw [Option.isSome_iff_exists] at t2_root_some; rcases t2_root_some with ⟨t2_root, t2_root_eq⟩
-      rw [FiniteDegreeTree.IsSuffix_iff] at suffix
-      rcases suffix with ⟨ms, suffix⟩
-      rw [← suffix]
-      intro trg
+          . exact node_eq
+          . apply ns_max
+            apply h.right
+            simp
+      . intro m
+        rw [PossiblyInfiniteList.tail_drop, PossiblyInfiniteList.get?_drop, ← PossiblyInfiniteList.head_drop]
+        rw [branch_eq2]
+        rw [FiniteDegreeTree.root_drop]
+        rw [h.right _ (by omega)]
+        simp
+    | inr h =>
+      have h : ∀ n, td.tree.get? (ns.take n) ≠ none := by
+        intro n contra
+        induction n with
+        | zero => rw [InfiniteList.take_zero] at contra; rw [← FiniteDegreeTree.root_eq] at contra; have contra' := td.isSome_root; simp [contra] at contra'
+        | succ n ih =>
+          apply h
+          exists n
+          constructor
+          . exact ih
+          . intro m m_gt
+            rw [← FiniteDegreeTree.root_drop] at contra
+            simp only [FiniteDegreeTree.root] at contra
+            rw [← PossiblyInfiniteTree.empty_iff_root_none] at contra
+            rw [gt_iff_lt, ← Nat.succ_le_iff] at m_gt
+            rcases Nat.exists_eq_add_of_le m_gt with ⟨K, m_gt⟩
+            rw [m_gt, InfiniteList.take_add, ← FiniteDegreeTree.get?_drop]
+            simp only [FiniteDegreeTree.get?]
+            rw [contra, PossiblyInfiniteTree.get?_empty]
       rcases td.fairness_infinite_branches trg with ⟨i, fairness⟩
       exists i
-      intro ns ns_length
-      rw [FiniteDegreeTree.get?_drop]
-      apply fairness (ms ++ ns)
-      rw [List.length_append, ge_iff_le]
-      apply Nat.le_add_left_of_le
-      exact ns_length
+      constructor
+      . rcases Option.ne_none_iff_exists'.mp (h i) with ⟨node, node_eq⟩
+        rw [branch_eq2]
+        exists node
+        constructor
+        . rw [FiniteDegreeTree.root_drop]
+          exact node_eq
+        . specialize fairness (ns.take i) (by rw [InfiniteList.length_take]; simp)
+          apply fairness
+          exact node_eq
+      . intro m
+        rw [PossiblyInfiniteList.tail_drop, PossiblyInfiniteList.get?_drop, ← PossiblyInfiniteList.head_drop]
+        rw [branch_eq2]
+        rw [FiniteDegreeTree.root_drop]
+        apply fairness
+        rw [InfiniteList.length_take]
+        omega
+}
 
-  def root (td : TreeDerivation obs rules) : ChaseNode obs rules := td.tree.root.get (td.isSome_root)
-  theorem root_mem {td : TreeDerivation obs rules} : td.root ∈ td := by exists []; simp [root, FiniteDegreeTree.root_eq, FiniteDegreeTree.get?, PossiblyInfiniteTree.get?]
+/-- The branches of the `TreeDerivation` are defined as all the `ChaseDerivation` that occur as branches in the tree. -/
+def branches (td : TreeDerivation obs rules) : Set (ChaseDerivation obs rules) := fun branch =>
+  branch.branch ∈ td.tree.branches
 
-  structure NodeWithAddress (td : TreeDerivation obs rules) where
-    node : ChaseNode obs rules
-    address : List Nat
-    eq : td.tree.get? address = some node
+/-- Each `ChaseDerivation` constructed using `derivation_for_branch` occurs in `branches`. -/
+theorem derivation_for_branch_mem_branches {td : TreeDerivation obs rules} {branch : PossiblyInfiniteList (ChaseNode obs rules)} {branch_mem : branch ∈ td.tree.branches} :
+  td.derivation_for_branch branch branch_mem ∈ td.branches := branch_mem
 
-  def subderivation_for_NodeWithAddress {td : TreeDerivation obs rules} (node : NodeWithAddress td) : TreeDerivation obs rules :=
-    td.derivation_for_suffix (td.tree.drop node.address) (td.tree.IsSuffix_drop node.address) (by simp [FiniteDegreeTree.root_drop, node.eq])
+/-- The result is the set of `FactSet`s that correspond to the results of the `branches`. -/
+def result (td : TreeDerivation obs rules) : Set (FactSet sig) := td.branches.map ChaseDerivation.result
 
-  theorem IsSuffix_subderivation_for_NodeWithAddress {td : TreeDerivation obs rules} {node : NodeWithAddress td} : td.subderivation_for_NodeWithAddress node <:+ td := td.tree.IsSuffix_drop node.address
+/-- Each element of the `result` models the rules. -/
+theorem result_models_rules {td : TreeDerivation obs rules} : ∀ fs ∈ td.result, fs.modelsRules rules := by
+  rintro fs ⟨branch, _, fs_mem⟩; rw [fs_mem]; apply branch.result_models_rules
 
-  def NodeWithAddress.cast_for_new_root_node
-      {td : TreeDerivation obs rules}
-      (new_root : NodeWithAddress td)
-      (node : (td.subderivation_for_NodeWithAddress new_root).NodeWithAddress) :
-      NodeWithAddress td where
-    node := node.node
-    address := new_root.address ++ node.address
-    eq := by
-      rw [← node.eq]
-      simp only [subderivation_for_NodeWithAddress, derivation_for_suffix, FiniteDegreeTree.get?_drop]
+end BranchesAndResult
 
-  theorem NodeWithAddress.mem {td : TreeDerivation obs rules} (node : td.NodeWithAddress) : node.node ∈ td := by exists node.address; exact node.eq
-  theorem NodeWithAddress.eq_of_address_eq {td : TreeDerivation obs rules} {n1 n2 : td.NodeWithAddress} : n1.address = n2.address -> n1 = n2 := by
-    intro eq
-    rw [NodeWithAddress.mk.injEq]
-    simp only [eq, and_true]
-    have eq1 := n1.eq
-    have eq2 := n2.eq
-    rw [eq] at eq1
-    rw [eq1, Option.some_inj] at eq2
-    exact eq2
+section TermsInChase
 
-  def root_NodeWithAddress (td : TreeDerivation obs rules) : NodeWithAddress td where
-    node := td.root
-    address := []
-    eq := by simp [root, FiniteDegreeTree.root_eq]
+/-!
+## Terms in the Chase
 
-  theorem root_NodeWithAddress_subderivation_for_NodeWithAddress {td : TreeDerivation obs rules} {node : NodeWithAddress td} : (td.subderivation_for_NodeWithAddress node).root_NodeWithAddress = { node := node.node, address := [], eq := by simp only [subderivation_for_NodeWithAddress, derivation_for_suffix, FiniteDegreeTree.get?_drop, List.append_nil]; exact node.eq } := by
-    simp [subderivation_for_NodeWithAddress, derivation_for_suffix, root_NodeWithAddress, root, FiniteDegreeTree.root_drop, node.eq]
+We make some general observations about certain terms that might occur in the chase.
 
-  theorem root_subderivation_for_NodeWithAddress {td : TreeDerivation obs rules} {node : NodeWithAddress td}: (td.subderivation_for_NodeWithAddress node).root = node.node := by
-    simp [subderivation_for_NodeWithAddress, derivation_for_suffix, root, FiniteDegreeTree.root_drop, node.eq]
+1. Constants can only originate directly from rules or from the initial fact set. No other constants can be introduced.
+2. Functional terms can either also originate from the initial fact set or they are introduced as fresh terms by a trigger.
 
-  def predecessor {td : TreeDerivation obs rules} (n1 n2 : NodeWithAddress td) : Prop := n1.address <+: n2.address
-  infixl:50 " ≼ " => predecessor
+The second observation entails that the precense of a functional term that does not occur in the initial fact set implies
+that the trigger that introduces this term must have been applied in some node.
+-/
 
-  theorem predecessor_refl {td : TreeDerivation obs rules} {node : NodeWithAddress td} : node ≼ node := List.prefix_rfl
-  theorem predecessor_trans {td : TreeDerivation obs rules} {n1 n2 n3 : NodeWithAddress td} : n1 ≼ n2 -> n2 ≼ n3 -> n1 ≼ n3 := List.IsPrefix.trans
-  theorem predecessor_antisymm {td : TreeDerivation obs rules} {n1 n2 : NodeWithAddress td} : n1 ≼ n2 -> n2 ≼ n1 -> n1 = n2 := by
-    rintro prefix1 ⟨addr2, prefix2⟩
-    apply NodeWithAddress.eq_of_address_eq
-    apply List.IsPrefix.eq_of_length_le prefix1
-    simp [← prefix2]
-  theorem predecessor_of_suffix {td : TreeDerivation obs rules} {new_root : NodeWithAddress td} {n1 n2 : NodeWithAddress (subderivation_for_NodeWithAddress new_root)} : n1 ≼ n2 -> (new_root.cast_for_new_root_node n1) ≼ (new_root.cast_for_new_root_node n2) := by
-    rintro ⟨addr, eq⟩
-    exists addr
+/-- Constants in the chase can only come from the initial fact set or from a constant in a rule. -/
+theorem constants_node_subset_constants_fs_union_constants_rules {td : TreeDerivation obs rules} {node : ChaseNode obs rules} (node_mem : node ∈ td) :
+    node.facts.constants ⊆ (td.root.facts.constants ∪ rules.head_constants) := by
+  rcases node_mem with ⟨addr, node_mem⟩
+  let node' : td.NodeWithAddress := {node := node, address := addr, eq := node_mem}
+  show node'.node.facts.constants ⊆ (td.root.facts.constants ∪ rules.head_constants)
+  induction node' using mem_rec_address with
+  | root =>
+    apply Set.subset_union_of_subset_left
+    apply Set.subset_refl
+  | step new_root ih c c_mem =>
     simp only [NodeWithAddress.cast_for_new_root_node]
-    simp [← eq]
-
-  def childTrees (td : TreeDerivation obs rules) : List (TreeDerivation obs rules) :=
-    td.tree.childTrees.attach.map (fun t =>
-      td.derivation_for_suffix t.val (by apply FiniteDegreeTree.IsSuffix_of_mem_childTrees; exact t.property) (by rw [Option.isSome_iff_ne_none]; exact t.val.property)
-    )
-
-  theorem mem_childTrees_iff {td : TreeDerivation obs rules} : ∀ c, c ∈ td.childTrees ↔ c.toFiniteDegreeTreeWithRoot ∈ td.tree.childTrees := by
-    intro c
-    unfold childTrees toFiniteDegreeTreeWithRoot derivation_for_suffix
-    simp only [List.mem_map, List.mem_attach, true_and]
-    constructor
-    . rintro ⟨d, eq⟩; rw [← eq]; exact d.property
-    . intro mem; exists ⟨c.toFiniteDegreeTreeWithRoot, mem⟩
-
-  theorem IsSuffix_of_mem_childTrees {td : TreeDerivation obs rules} : ∀ td2 ∈ td.childTrees, td2 <:+ td := by intro td2 mem; apply FiniteDegreeTree.IsSuffix_of_mem_childTrees td2.toFiniteDegreeTreeWithRoot; rw [← mem_childTrees_iff]; exact mem
-
-  theorem suffix_iff_eq_or_suffix_childTree {td1 td2 : TreeDerivation obs rules} : td1 <:+ td2 ↔ td1 = td2 ∨ ∃ td3 ∈ td2.childTrees, td1 <:+ td3 := by
-    constructor
-    . rw [IsSuffix_iff, FiniteDegreeTree.IsSuffix_iff]; rintro ⟨ns, suffix⟩
-      cases ns with
-      | nil => apply Or.inl; rw [TreeDerivation.mk.injEq]; rw [FiniteDegreeTree.drop_nil] at suffix; apply Eq.symm; exact suffix
-      | cons hd tl =>
-        apply Or.inr
-        cases eq : td2.childTrees[hd]? with
-        | none =>
-          have contra := td1.isSome_root
-          rw [Option.isSome_iff_ne_none] at contra
-          apply False.elim; apply contra
-          have suf : td1.tree <:+ td2.tree.drop [hd] := by
-            rw [FiniteDegreeTree.IsSuffix_iff]
-            exists tl
-          rw [← FiniteDegreeTree.empty_iff_root_none]
-          simp only [childTrees, List.getElem?_map, List.getElem?_attach, Option.map_eq_none_iff, Option.pmap_eq_none_iff] at eq
-          rw [FiniteDegreeTree.get?_childTrees, FiniteDegreeTree.FiniteDegreeTreeWithRoot.tree_to_opt_none_iff] at eq
-          rw [← FiniteDegreeTree.empty_iff_root_none] at eq
-          rw [eq] at suf
-          apply FiniteDegreeTree.empty_suffix_of_empty suf
-        | some c =>
-          rw [List.getElem?_eq_some_iff] at eq
-          rcases eq with ⟨_, eq⟩
-          exists c
-          constructor
-          . simp [← eq]
-          . rw [IsSuffix_iff, FiniteDegreeTree.IsSuffix_iff]; exists tl; rw [← eq]; simp only [childTrees, derivation_for_suffix, List.getElem_map, List.getElem_attach, FiniteDegreeTree.get_childTrees]; exact suffix
-    . intro h; cases h with
-      | inl eq => rw [eq]; exact FiniteDegreeTree.IsSuffix_refl
-      | inr suffix => rcases suffix with ⟨td3, td3_mem, suffix⟩; apply FiniteDegreeTree.IsSuffix_trans suffix; exact IsSuffix_of_mem_childTrees _ td3_mem
-
-  def childNodes (td : TreeDerivation obs rules) : List (ChaseNode obs rules) := td.tree.childNodes
-
-  def childNodes_as_NodesWithAddress (td : TreeDerivation obs rules) : List (NodeWithAddress td) := td.childNodes.zipIdx_with_lt.attach.map (fun ⟨⟨c, idx⟩, prop⟩ => {
-    node := c
-    address := [idx.val]
-    eq := by
-      rw [List.mem_zipIdx_with_lt_iff_mem_zipIdx, List.mem_zipIdx_iff_getElem?] at prop
-      simp only [childNodes, FiniteDegreeTree.get?_childNodes, FiniteDegreeTree.get?_childTrees, FiniteDegreeTree.FiniteDegreeTreeWithRoot.opt_to_tree_after_tree_to_opt] at prop
-      exact prop
-  })
-
-  theorem length_childNodes_as_Nodes {td : TreeDerivation obs rules} : td.childNodes_as_NodesWithAddress.length = td.childNodes.length := by
-    simp [childNodes_as_NodesWithAddress, List.length_zipIdx_with_lt]
-
-  theorem childNodes_as_NodesWithAddress_eq_childNodes {td : TreeDerivation obs rules} : td.childNodes = td.childNodes_as_NodesWithAddress.map NodeWithAddress.node := by
-    apply List.ext_getElem
-    . rw [List.length_map, td.length_childNodes_as_Nodes]
-    intro i _ _
-    simp only [childNodes_as_NodesWithAddress, List.getElem_map, List.getElem_attach]
-    rw [List.zipIdx_with_lt_getElem_fst_eq_getElem]
-
-  theorem node_getElem_childNodes_as_nodesWithAddress {td : TreeDerivation obs rules} : ∀ i (lt : i < td.childNodes_as_NodesWithAddress.length), td.childNodes_as_NodesWithAddress[i].node = td.childNodes[i]'(by rw [← length_childNodes_as_Nodes]; exact lt) := by simp [childNodes_as_NodesWithAddress_eq_childNodes]
-
-  theorem mem_childNodes_of_mem_childNodes_as_NodesWithAddress {td : TreeDerivation obs rules} : ∀ {n}, n ∈ td.childNodes_as_NodesWithAddress -> n.node ∈ td.childNodes := by
-    intro n n_mem; rw [childNodes_as_NodesWithAddress_eq_childNodes]; apply List.mem_map_of_mem; exact n_mem
-
-  theorem childNodes_eq {td : TreeDerivation obs rules} : td.childNodes = td.childTrees.map root := by
-    unfold childNodes childTrees
-    rw [FiniteDegreeTree.childNodes_eq]
-    apply List.ext_getElem
-    . simp
-    . intro i _ _; simp [derivation_for_suffix, root]
-
-  theorem subderivation_mem_childTrees_of_mem_childNodes_as_NodesWithAddress {td : TreeDerivation obs rules} {node : NodeWithAddress td} :
-      node ∈ td.childNodes_as_NodesWithAddress -> (td.subderivation_for_NodeWithAddress node) ∈ td.childTrees := by
-    intro node_mem
-    simp only [childNodes_as_NodesWithAddress, List.mem_map, List.mem_attach, true_and] at node_mem
-    rcases node_mem with ⟨⟨node_with_idx, node_mem⟩, node_eq⟩
-    rw [List.mem_zipIdx_with_lt_iff_mem_zipIdx] at node_mem
-    have node_mem := List.mem_zipIdx' node_mem
-    have : subderivation_for_NodeWithAddress node = td.childTrees[node_with_idx.snd.val]'(by have lt := node_with_idx.snd.isLt; simp only [childNodes_eq, List.length_map] at lt; exact lt) := by
-      simp only [childTrees, List.getElem_map, List.getElem_attach, FiniteDegreeTree.get_childTrees]
-      simp only [subderivation_for_NodeWithAddress]
-      rw [← node_eq]
-    rw [this]
-    apply List.getElem_mem
-
-  theorem mem_of_mem_childNodes {td : TreeDerivation obs rules} : ∀ n ∈ td.childNodes, n ∈ td := FiniteDegreeTree.mem_of_mem_childNodes
-
-  theorem isSome_origin_of_mem_childNodes {td : TreeDerivation obs rules} : ∀ n ∈ td.childNodes, n.origin.isSome := by
-    intro n n_mem
-    have trg_ex := td.triggers_exist []
-    rw [FiniteDegreeTree.drop_nil] at trg_ex
-    specialize trg_ex td.root (by simp [root])
-    cases trg_ex with
-    | inl trg_ex => rcases trg_ex with ⟨_, _, trg_ex⟩; unfold childNodes at n_mem; rw [trg_ex] at n_mem; simp only [List.mem_map] at n_mem; rcases n_mem with ⟨a, _, eq⟩; rw [← eq]; simp
-    | inr trg_ex => have contra := trg_ex.right; unfold childNodes at n_mem; rw [contra] at n_mem; simp at n_mem
-
-  theorem active_trigger_origin_of_mem_childNodes {td : TreeDerivation obs rules} :
-      ∀ {n}, (mem : n ∈ td.childNodes) -> (n.origin.get (td.isSome_origin_of_mem_childNodes _ mem)).fst.val.active td.root.facts := by
-    intro n n_mem
-    have trg_ex := td.triggers_exist []
-    rw [FiniteDegreeTree.drop_nil] at trg_ex
-    specialize trg_ex td.root (by simp [root])
-    cases trg_ex with
-    | inl trg_ex => rcases trg_ex with ⟨_, trg_act, trg_ex⟩; unfold childNodes at n_mem; rw [trg_ex] at n_mem; simp only [List.mem_map] at n_mem; rcases n_mem with ⟨a, _, eq⟩; simp only [← eq]; exact trg_act
-    | inr trg_ex => have contra := trg_ex.right; unfold childNodes at n_mem; rw [contra] at n_mem; simp at n_mem
-
-  theorem childNodes_ne_nil_iff_trg_ex {td : TreeDerivation obs rules} : td.childNodes ≠ [] ↔ ∃ (trg : RTrigger obs rules), trg.val.active td.root.facts := by
-    constructor
-    . rw [List.ne_nil_iff_exists_cons]
-      rintro ⟨hd, tl, eq⟩
-      exists (hd.origin.get (td.isSome_origin_of_mem_childNodes _ (by simp [eq]))).fst
-      apply active_trigger_origin_of_mem_childNodes
-      simp [eq]
-    . rintro ⟨trg, active⟩
-      intro eq_nil
-      apply td.fairness_leaves td.root _ trg active
-      exists []
-      simp only [root, Option.some_get, FiniteDegreeTree.root, PossiblyInfiniteTree.root_eq, true_and]
-      simp only [childNodes, FiniteDegreeTree.childNodes, PossiblyInfiniteList.toList_of_finite_empty_iff] at eq_nil
-      simp only [PossiblyInfiniteTree.drop_nil]
-      rw [← PossiblyInfiniteList.empty_iff_head_none]
-      exact eq_nil
-
-  theorem facts_childNodes {td : TreeDerivation obs rules} :
-      ∀ {n}, (mem : n ∈ td.childNodes) -> n.facts = td.root.facts ∪ (n.origin_result (td.isSome_origin_of_mem_childNodes _ mem)).toSet := by
-    intro n n_mem
-    have trg_ex := td.triggers_exist []
-    rw [FiniteDegreeTree.drop_nil] at trg_ex
-    specialize trg_ex td.root (by simp [root])
-    cases trg_ex with
-    | inl trg_ex =>
-      rcases trg_ex with ⟨trg, trg_act, trg_ex⟩; unfold childNodes at n_mem; rw [trg_ex] at n_mem; simp only [List.mem_map] at n_mem
-      rcases n_mem with ⟨head, _, eq⟩; simp only [← eq]
-      have head_mem := head.property
-      rw [List.mem_zipIdx_with_lt_iff_mem_zipIdx, List.mem_zipIdx_iff_getElem?, List.getElem?_eq_some_iff] at head_mem
-      rcases head_mem with ⟨_, head_mem⟩
-      simp only at head_mem
-      simp only [← head_mem]
-      rfl
-    | inr trg_ex => have contra := trg_ex.right; unfold childNodes at n_mem; rw [contra] at n_mem; simp at n_mem
-
-  theorem root_prec_childNodes {td : TreeDerivation obs rules} : ∀ n ∈ td.childNodes_as_NodesWithAddress, td.root_NodeWithAddress ≼ n := by
-    intros; exact List.nil_prefix
-
-  theorem mem_rec_address
-      {td : TreeDerivation obs rules}
-      {motive : NodeWithAddress td -> Prop}
-      (root : motive td.root_NodeWithAddress)
-      (step : ∀ (new_root : NodeWithAddress td), motive new_root -> ∀ c, (mem : c ∈ (td.subderivation_for_NodeWithAddress new_root).childNodes_as_NodesWithAddress) -> motive (NodeWithAddress.cast_for_new_root_node new_root c))
-      (node : NodeWithAddress td) :
-      motive node := by
-    let motive' (rev_addr : List Nat) := ∀ n, (mem : n ∈ td.tree.get? rev_addr.reverse) -> motive {
-      node := n
-      address := rev_addr.reverse
-      eq := mem
-    }
-    let rev_addr_node := node.address.reverse
-    have : motive' rev_addr_node := by
-      induction rev_addr_node with
-      | nil =>
-        intro n n_mem
-        have eq : td.root_NodeWithAddress = {node := n, address := [].reverse, eq := n_mem} := by apply NodeWithAddress.eq_of_address_eq; simp [root_NodeWithAddress]
-        rw [← eq]
-        exact root
-      | cons hd tl ih =>
-        intro n n_mem
-        cases eq : td.tree.get? tl.reverse with
-        | none =>
-          have contra := td.tree.no_orphans (td.tree.drop tl.reverse) (FiniteDegreeTree.IsSuffix_drop tl.reverse) (by rw [FiniteDegreeTree.root_drop]; exact eq)
-          have n_mem : n ∈ (td.tree.drop tl.reverse).childNodes[hd]? := by
-            rw [FiniteDegreeTree.get?_childNodes, FiniteDegreeTree.get?_childTrees, FiniteDegreeTree.FiniteDegreeTreeWithRoot.opt_to_tree_after_tree_to_opt]
-            rw [FiniteDegreeTree.drop_drop, FiniteDegreeTree.root_drop]
-            rw [List.reverse_cons] at n_mem
-            exact n_mem
-          simp [contra] at n_mem
-        | some m =>
-          have n_mem : n ∈ (td.tree.drop tl.reverse).childNodes[hd]? := by rw [FiniteDegreeTree.get?_childNodes, FiniteDegreeTree.get?_childTrees, FiniteDegreeTree.FiniteDegreeTreeWithRoot.opt_to_tree_after_tree_to_opt, FiniteDegreeTree.root_drop, FiniteDegreeTree.get?_drop]; rw [List.reverse_cons] at n_mem; exact n_mem
-          let new_root : td.NodeWithAddress := { node := m, address := tl.reverse, eq := eq }
-          specialize step new_root (ih m eq) _ (by
-            simp only [childNodes_as_NodesWithAddress, List.mem_map]
-            exists ⟨⟨n, ⟨hd, by
-                simp only [subderivation_for_NodeWithAddress, derivation_for_suffix, childNodes, new_root]
-                rw [Option.mem_def, List.getElem?_eq_some_iff] at n_mem
-                rcases n_mem with ⟨lt, _⟩
-                exact lt⟩⟩, by
-              rw [List.mem_zipIdx_with_lt_iff_mem_zipIdx, List.mem_zipIdx_iff_getElem?]
-              simp only [subderivation_for_NodeWithAddress, derivation_for_suffix, childNodes, new_root]
-              exact n_mem⟩
-            constructor; simp; rfl)
-          simp only [NodeWithAddress.cast_for_new_root_node, new_root] at step
-          simp only [List.reverse_cons]
-          exact step
-    specialize this node.node (by simp only [rev_addr_node, List.reverse_reverse]; exact node.eq)
-    simp only [rev_addr_node, List.reverse_reverse] at this
-    exact this
-
-  theorem mem_some_childTree_iff {td : TreeDerivation obs rules} {node : ChaseNode obs rules} :
-      (∃ t ∈ td.childTrees, node ∈ t) ↔ ∃ td2, td2 <:+ td ∧ node ∈ td2.childNodes := by
-    constructor
-    . rintro ⟨t, t_mem, node_mem⟩
-      rcases node_mem with ⟨addr, node_mem⟩
-      let node' : t.NodeWithAddress := { node := node, address := addr, eq := node_mem }
-      show ∃ td2, td2 <:+ td ∧ node'.node ∈ td2.childNodes
-      induction node' using mem_rec_address with
-      | root => exists td; constructor; exact td.tree.IsSuffix_refl; simp only [childNodes_eq, root_NodeWithAddress]; apply List.mem_map_of_mem; exact t_mem
-      | step new_root ih c c_mem =>
-        exists subderivation_for_NodeWithAddress new_root; constructor
-        . apply FiniteDegreeTree.IsSuffix_trans IsSuffix_subderivation_for_NodeWithAddress; exact IsSuffix_of_mem_childTrees _ t_mem
-        . rw [childNodes_as_NodesWithAddress_eq_childNodes]; apply List.mem_map_of_mem; exact c_mem
-    . rintro ⟨td2, suffix, node_mem⟩
-      rw [IsSuffix_iff, FiniteDegreeTree.IsSuffix_iff] at suffix; rcases suffix with ⟨ns, suffix⟩
-      cases ns with
-      | nil =>
-        have : td = td2 := by rw [TreeDerivation.mk.injEq]; rw [FiniteDegreeTree.drop_nil] at suffix; exact suffix
-        rw [childNodes_eq, List.mem_map] at node_mem; rcases node_mem with ⟨t, t_mem, node_mem⟩; exists t; constructor; rw [this]; exact t_mem; rw [← node_mem]; exact root_mem
-      | cons hd tl =>
-        cases eq : td.childTrees[hd]? with
-        | none =>
-          have contra := td2.isSome_root
-          rw [Option.isSome_iff_ne_none] at contra
-          apply False.elim; apply contra
-          have suf : td2.tree <:+ td.tree.drop [hd] := by
-            rw [FiniteDegreeTree.IsSuffix_iff]
-            exists tl
-          rw [← FiniteDegreeTree.empty_iff_root_none]
-          simp only [childTrees, List.getElem?_map, List.getElem?_attach, Option.map_eq_none_iff, Option.pmap_eq_none_iff] at eq
-          rw [FiniteDegreeTree.get?_childTrees, FiniteDegreeTree.FiniteDegreeTreeWithRoot.tree_to_opt_none_iff] at eq
-          rw [← FiniteDegreeTree.empty_iff_root_none] at eq
-          rw [eq] at suf
-          apply FiniteDegreeTree.empty_suffix_of_empty suf
-        | some t =>
-          rw [List.getElem?_eq_some_iff] at eq; rcases eq with ⟨_, eq⟩
-          exists t; constructor; simp [← eq]
-          have : td2 <:+ t := by rw [IsSuffix_iff, FiniteDegreeTree.IsSuffix_iff]; exists tl; rw [← eq]; simp only [childTrees, derivation_for_suffix, List.getElem_map, List.getElem_attach, FiniteDegreeTree.get_childTrees]; rw [FiniteDegreeTree.drop_drop, List.singleton_append]; exact suffix
-          apply mem_of_mem_suffix this
-          apply mem_of_mem_childNodes
-          exact node_mem
-
-  theorem facts_node_subset_every_mem {td : TreeDerivation obs rules} : ∀ node ∈ td, td.root.facts ⊆ node.facts := by
-    rintro node ⟨addr, node_mem⟩
-    let node' : td.NodeWithAddress := { node := node, address := addr, eq := node_mem }
-    show td.root.facts ⊆ node'.node.facts
-    induction node' using mem_rec_address with
-    | root => apply Set.subset_refl
-    | step new_root ih c c_mem =>
-      apply Set.subset_trans ih
-      simp only [NodeWithAddress.cast_for_new_root_node]
-      rw [facts_childNodes (mem_childNodes_of_mem_childNodes_as_NodesWithAddress c_mem)]
-      apply Set.subset_union_of_subset_left
-      rw [root_subderivation_for_NodeWithAddress]
-      apply Set.subset_refl
-
-  theorem facts_node_subset_of_prec {td : TreeDerivation obs rules} {node1 node2 : td.NodeWithAddress} : node1 ≼ node2 -> node1.node.facts ⊆ node2.node.facts := by
-    rintro ⟨diff, addr_eq⟩
-    have := (subderivation_for_NodeWithAddress node1).facts_node_subset_every_mem node2.node
-    rw [root_subderivation_for_NodeWithAddress] at this
-    apply this
-    exists diff
-    rw [← node2.eq, ← addr_eq]
-    rfl
-
-  theorem root_not_mem_childTrees {td : TreeDerivation obs rules} : ¬ ∃ t ∈ td.childTrees, td.root ∈ t := by
-    intro contra
-    rw [mem_some_childTree_iff] at contra
-    rcases contra with ⟨td2, suffix, contra⟩
-    apply (td2.active_trigger_origin_of_mem_childNodes contra).right
-    apply obs.contains_trg_result_implies_cond
-    apply Set.subset_trans (td.root.facts_contain_origin_result (td.root.origin.get (td2.isSome_origin_of_mem_childNodes _ contra)) (by simp))
-    apply td.facts_node_subset_every_mem
-    apply mem_of_mem_suffix suffix
-    exact td2.root_mem
-
-  theorem eq_of_suffix_of_root_mem {td1 td2 : TreeDerivation obs rules} (suffix : td1 <:+ td2) (root_mem : td2.root ∈ td1) : td1 = td2 := by
-    rw [suffix_iff_eq_or_suffix_childTree] at suffix
-    cases suffix with
-    | inl suffix => exact suffix
-    | inr suffix => rcases suffix with ⟨td3, td3_mem, suffix⟩; apply False.elim; apply td2.root_not_mem_childTrees; exists td3; constructor; exact td3_mem; apply mem_of_mem_suffix suffix; exact root_mem
-
-  theorem constants_node_subset_constants_fs_union_constants_rules {td : TreeDerivation obs rules} {node : ChaseNode obs rules} (node_mem : node ∈ td) :
-      node.facts.constants ⊆ (td.root.facts.constants ∪ rules.head_constants) := by
-    rcases node_mem with ⟨addr, node_mem⟩
-    let node' : td.NodeWithAddress := {node := node, address := addr, eq := node_mem}
-    show node'.node.facts.constants ⊆ (td.root.facts.constants ∪ rules.head_constants)
-    induction node' using mem_rec_address with
-    | root =>
-      apply Set.subset_union_of_subset_left
-      apply Set.subset_refl
-    | step new_root ih c c_mem =>
-      simp only [NodeWithAddress.cast_for_new_root_node]
-      rw [facts_childNodes (mem_childNodes_of_mem_childNodes_as_NodesWithAddress c_mem), root_subderivation_for_NodeWithAddress]
-      intro d d_mem
-      rw [FactSet.constants_union] at d_mem
-      cases d_mem with
-      | inl d_mem => apply ih; exact d_mem
-      | inr d_mem =>
-        let origin := c.node.origin.get (isSome_origin_of_mem_childNodes _ (mem_childNodes_of_mem_childNodes_as_NodesWithAddress c_mem))
-        apply Set.subset_trans (origin.fst.val.mapped_head_constants_subset origin.snd)
-        . intro d d_mem
-          rw [List.mem_toSet, List.mem_append] at d_mem
-          cases d_mem with
-          | inl d_mem =>
-            apply ih
-            rw [List.mem_flatMap] at d_mem
-            rcases d_mem with ⟨t, t_mem, d_mem⟩
-            rw [List.mem_map] at t_mem
-            rcases t_mem with ⟨v, v_mem, t_mem⟩
-            rcases FunctionFreeConjunction.mem_vars.mp (origin.fst.val.rule.frontier_subset_vars_body v_mem) with ⟨a, a_mem, v_mem'⟩
-            exists origin.fst.val.subs.apply_function_free_atom a
-            constructor
-            . have := active_trigger_origin_of_mem_childNodes (mem_childNodes_of_mem_childNodes_as_NodesWithAddress c_mem)
-              rw [root_subderivation_for_NodeWithAddress] at this
-              apply this.left
-              rw [List.mem_toSet]
-              unfold PreTrigger.mapped_body
-              unfold GroundSubstitution.apply_function_free_conj
-              apply List.mem_map_of_mem
-              exact a_mem
-            . unfold Fact.constants
-              rw [List.mem_flatMap]
-              exists t
-              constructor
-              . unfold GroundSubstitution.apply_function_free_atom
-                unfold TermMapping.apply_generalized_atom
-                rw [List.mem_map]
-                exists VarOrConst.var v
-                constructor
-                . exact v_mem'
-                . unfold PreTrigger.subs_for_mapped_head at t_mem
-                  rw [PreTrigger.apply_to_var_or_const_frontier_var] at t_mem
-                  . exact t_mem
-                  . exact v_mem
-              . exact d_mem
-          | inr d_mem =>
-            apply Or.inr
-            exists origin.fst.val.rule
-            constructor
-            . exact origin.fst.property
-            . unfold Rule.head_constants
-              rw [List.mem_flatMap]
-              exists origin.fst.val.rule.head[origin.snd.val]'(by rw [← PreTrigger.length_mapped_head]; exact origin.snd.isLt)
-              constructor
-              . apply List.get_mem
-              . exact d_mem
-        . exact d_mem
-
-  theorem result_models_rules {td : TreeDerivation obs rules} : ∀ fs ∈ td.result, fs.modelsRules rules := by
-    rintro fs ⟨branch, _, fs_mem⟩; rw [← fs_mem]; apply branch.result_models_rules
-
-  theorem functional_term_originates_from_some_trigger
-      {td : TreeDerivation obs rules}
-      (node : NodeWithAddress td)
-      {t : GroundTerm sig}
-      (t_is_func : ∃ func ts arity_ok, t = GroundTerm.func func ts arity_ok)
-      (t_mem : t ∈ node.node.facts.terms) :
-      t ∈ td.root.facts.terms ∨ ∃ node2, node2 ≼ node ∧ ∃ orig ∈ node2.node.origin, t ∈ orig.fst.val.fresh_terms_for_head_disjunct orig.snd.val (by rw [← PreTrigger.length_mapped_head]; exact orig.snd.isLt) := by
-    induction node using mem_rec_address with
-    | root => apply Or.inl; exact t_mem
-    | step new_root ih c c_mem =>
-      simp only [NodeWithAddress.cast_for_new_root_node] at t_mem
-      rw [facts_childNodes (mem_childNodes_of_mem_childNodes_as_NodesWithAddress c_mem), root_subderivation_for_NodeWithAddress, FactSet.terms_union] at t_mem
-
-      have aux : t ∈ new_root.node.facts.terms -> t ∈ td.root.facts.terms ∨ ∃ (node2 : td.NodeWithAddress), node2 ≼ (NodeWithAddress.cast_for_new_root_node new_root c) ∧ ∃ orig ∈ node2.node.origin, t ∈ orig.fst.val.fresh_terms_for_head_disjunct orig.snd.val (by rw [← PreTrigger.length_mapped_head]; exact orig.snd.isLt) := by
-        intro t_mem
-        cases ih t_mem with
-        | inl ih => apply Or.inl; exact ih
-        | inr ih =>
-          rcases ih with ⟨node2, prec, t_mem⟩
-          apply Or.inr; exists node2; constructor;
-          . apply predecessor_trans prec
-            have : new_root = new_root.cast_for_new_root_node (subderivation_for_NodeWithAddress new_root).root_NodeWithAddress := by
-              apply NodeWithAddress.eq_of_address_eq
-              rw [root_NodeWithAddress_subderivation_for_NodeWithAddress]
-              simp [NodeWithAddress.cast_for_new_root_node]
-            conv => left; rw [this]
-            apply predecessor_of_suffix
-            apply root_prec_childNodes
-            exact c_mem
-          . exact t_mem
-
-      cases t_mem with
-      | inl t_mem => exact aux t_mem
-      | inr t_mem =>
-        unfold ChaseNode.origin_result at t_mem
-        rw [FactSet.mem_terms_toSet, PreTrigger.mem_terms_mapped_head_iff] at t_mem
-        cases t_mem with
-        | inl t_mem => rcases t_is_func with ⟨func, ts, arity, t_is_func⟩; rcases t_mem with ⟨c, _, t_mem⟩; rw [← t_mem] at t_is_func; simp [GroundTerm.const, GroundTerm.func] at t_is_func
-        | inr t_mem =>
-        cases t_mem with
-        | inr t_mem =>
-          apply Or.inr; exists new_root.cast_for_new_root_node c; constructor
-          . exact predecessor_refl
-          . exists c.node.origin.get (isSome_origin_of_mem_childNodes _ (mem_childNodes_of_mem_childNodes_as_NodesWithAddress c_mem))
-            simp only [NodeWithAddress.cast_for_new_root_node, Option.get_mem, true_and]
-            exact t_mem
-        | inl t_mem =>
-          apply aux
-          have := active_trigger_origin_of_mem_childNodes (mem_childNodes_of_mem_childNodes_as_NodesWithAddress c_mem)
-          rw [root_subderivation_for_NodeWithAddress] at this
-          apply FactSet.terms_subset_of_subset this.left
+    rw [facts_childNodes (NodeWithAddress.mem_childNodes_of_mem_childNodes c_mem), NodeWithAddress.root_subderivation']
+    intro d d_mem
+    rw [FactSet.constants_union] at d_mem
+    cases d_mem with
+    | inl d_mem => apply ih; exact d_mem
+    | inr d_mem =>
+      let origin := c.node.origin.get (isSome_origin_of_mem_childNodes _ (NodeWithAddress.mem_childNodes_of_mem_childNodes c_mem))
+      apply Set.subset_trans (origin.fst.val.mapped_head_constants_subset origin.snd)
+      . intro d d_mem
+        rw [List.mem_toSet, List.mem_append] at d_mem
+        cases d_mem with
+        | inl d_mem =>
+          apply ih
+          rw [List.mem_flatMap] at d_mem
+          rcases d_mem with ⟨t, t_mem, d_mem⟩
           rw [List.mem_map] at t_mem
           rcases t_mem with ⟨v, v_mem, t_mem⟩
-          rw [FactSet.mem_terms_toSet, PreTrigger.mem_terms_mapped_body_iff]
+          rcases FunctionFreeConjunction.mem_vars.mp (origin.fst.val.rule.frontier_subset_vars_body v_mem) with ⟨a, a_mem, v_mem'⟩
+          exists origin.fst.val.subs.apply_function_free_atom a
+          constructor
+          . have := active_trigger_origin_of_mem_childNodes (NodeWithAddress.mem_childNodes_of_mem_childNodes c_mem)
+            rw [NodeWithAddress.root_subderivation'] at this
+            apply this.left
+            rw [List.mem_toSet]
+            unfold PreTrigger.mapped_body
+            unfold GroundSubstitution.apply_function_free_conj
+            apply List.mem_map_of_mem
+            exact a_mem
+          . unfold Fact.constants
+            rw [List.mem_flatMap]
+            exists t
+            constructor
+            . unfold GroundSubstitution.apply_function_free_atom
+              unfold TermMapping.apply_generalized_atom
+              rw [List.mem_map]
+              exists VarOrConst.var v
+              constructor
+              . exact v_mem'
+              . unfold PreTrigger.subs_for_mapped_head at t_mem
+                rw [PreTrigger.apply_to_var_or_const_frontier_var] at t_mem
+                . exact t_mem
+                . exact v_mem
+            . exact d_mem
+        | inr d_mem =>
           apply Or.inr
-          exists v; simp only [t_mem, and_true]
-          apply Rule.frontier_subset_vars_body; rw [Rule.mem_frontier_iff_mem_frontier_for_head]; exact ⟨_, v_mem⟩
+          exists origin.fst.val.rule
+          constructor
+          . exact origin.fst.property
+          . unfold Rule.head_constants
+            rw [List.mem_flatMap]
+            exists origin.fst.val.rule.head[origin.snd.val]'(by rw [← PreTrigger.length_mapped_head]; exact origin.snd.isLt)
+            constructor
+            . apply List.get_mem
+            . exact d_mem
+      . exact d_mem
 
-  theorem trigger_introducing_functional_term_occurs_in_chase
-      {td : TreeDerivation obs rules}
-      (node : NodeWithAddress td)
-      {t : GroundTerm sig}
-      (t_mem_node : t ∈ node.node.facts.terms)
-      {trg : RTrigger obs rules}
-      {disj_idx : Nat}
-      {lt : disj_idx < trg.val.rule.head.length}
-      (t_mem_trg : t ∈ trg.val.fresh_terms_for_head_disjunct disj_idx lt) :
-      t ∈ td.root.facts.terms ∨ ∃ node2, node2 ≼ node ∧ ∃ orig ∈ node2.node.origin, orig.fst.equiv trg ∧ orig.snd.val = disj_idx := by
-    cases functional_term_originates_from_some_trigger node (by
-      cases eq : t with
-      | const _ =>
-        rw [eq] at t_mem_trg
-        simp [PreTrigger.fresh_terms_for_head_disjunct, PreTrigger.functional_term_for_var, GroundTerm.func, GroundTerm.const] at t_mem_trg
-      | func func ts arity_ok => exists func, ts, arity_ok
-    ) t_mem_node with
-    | inl t_mem => apply Or.inl; exact t_mem
-    | inr t_mem =>
-      apply Or.inr
-      rcases t_mem with ⟨node2, prec, origin, origin_eq, t_mem⟩
-      exists node2; simp only [prec, true_and]
-      exists origin; simp only [origin_eq, true_and]
-      exact RTrigger.equiv_of_term_mem_fresh_terms_for_head_disjunct t_mem t_mem_trg
+/-- Each functional term in the chase originates as a fresh term from a trigger if it was not already part of the initial fact set. -/
+theorem functional_term_originates_from_some_trigger
+    {td : TreeDerivation obs rules}
+    (node : NodeWithAddress td)
+    {t : GroundTerm sig}
+    (t_is_func : ∃ func ts arity_ok, t = GroundTerm.func func ts arity_ok)
+    (t_mem : t ∈ node.node.facts.terms) :
+    t ∈ td.root.facts.terms ∨ ∃ node2, node2 ≼ node ∧ ∃ orig ∈ node2.node.origin, t ∈ orig.fst.val.fresh_terms_for_head_disjunct orig.snd.val (by rw [← PreTrigger.length_mapped_head]; exact orig.snd.isLt) := by
+  induction node using mem_rec_address with
+  | root => apply Or.inl; exact t_mem
+  | step new_root ih c c_mem =>
+    simp only [NodeWithAddress.cast_for_new_root_node] at t_mem
+    rw [facts_childNodes (NodeWithAddress.mem_childNodes_of_mem_childNodes c_mem), NodeWithAddress.root_subderivation', FactSet.terms_union] at t_mem
 
-  theorem result_of_trigger_introducing_functional_term_occurs_in_chase
-      {td : TreeDerivation obs rules}
-      (node : NodeWithAddress td)
-      {t : GroundTerm sig}
-      (t_mem_node : t ∈ node.node.facts.terms)
-      {trg : RTrigger obs rules}
-      {disj_idx : Nat}
-      {lt : disj_idx < trg.val.rule.head.length}
-      (t_mem_trg : t ∈ trg.val.fresh_terms_for_head_disjunct disj_idx lt) :
-      t ∈ td.root.facts.terms ∨ (trg.val.mapped_head[disj_idx]'(by rw [PreTrigger.length_mapped_head]; exact lt)).toSet ⊆ node.node.facts := by
-    cases trigger_introducing_functional_term_occurs_in_chase node t_mem_node t_mem_trg with
-    | inl t_mem => apply Or.inl; exact t_mem
+    have aux : t ∈ new_root.node.facts.terms -> t ∈ td.root.facts.terms ∨ ∃ (node2 : td.NodeWithAddress), node2 ≼ (NodeWithAddress.cast_for_new_root_node new_root c) ∧ ∃ orig ∈ node2.node.origin, t ∈ orig.fst.val.fresh_terms_for_head_disjunct orig.snd.val (by rw [← PreTrigger.length_mapped_head]; exact orig.snd.isLt) := by
+      intro t_mem
+      cases ih t_mem with
+      | inl ih => apply Or.inl; exact ih
+      | inr ih =>
+        rcases ih with ⟨node2, prec, t_mem⟩
+        apply Or.inr; exists node2; constructor;
+        . apply predecessor_trans prec
+          have : new_root = new_root.cast_for_new_root_node (NodeWithAddress.root new_root.subderivation) := by
+            apply NodeWithAddress.eq_of_address_eq
+            rw [NodeWithAddress.root_subderivation]
+            simp [NodeWithAddress.cast_for_new_root_node]
+          conv => left; rw [this]
+          apply predecessor_of_suffix
+          apply root_prec_childNodes
+          exact c_mem
+        . exact t_mem
+
+    cases t_mem with
+    | inl t_mem => exact aux t_mem
     | inr t_mem =>
-      apply Or.inr
-      rcases t_mem with ⟨node2, prec, origin, origin_eq, equiv, index_eq⟩
-      apply Set.subset_trans _ (td.facts_node_subset_of_prec prec)
-      simp only [← PreTrigger.result_eq_of_equiv equiv, ← index_eq]
-      exact node2.node.facts_contain_origin_result _ origin_eq
+      unfold ChaseNode.origin_result at t_mem
+      rw [FactSet.mem_terms_toSet, PreTrigger.mem_terms_mapped_head_iff] at t_mem
+      cases t_mem with
+      | inl t_mem => rcases t_is_func with ⟨func, ts, arity, t_is_func⟩; rcases t_mem with ⟨c, _, t_mem⟩; rw [← t_mem] at t_is_func; simp [GroundTerm.const, GroundTerm.func] at t_is_func
+      | inr t_mem =>
+      cases t_mem with
+      | inr t_mem =>
+        apply Or.inr; exists new_root.cast_for_new_root_node c; constructor
+        . exact predecessor_refl
+        . exists c.node.origin.get (isSome_origin_of_mem_childNodes _ (NodeWithAddress.mem_childNodes_of_mem_childNodes c_mem))
+          simp only [NodeWithAddress.cast_for_new_root_node, Option.get_mem, true_and]
+          exact t_mem
+      | inl t_mem =>
+        apply aux
+        have := active_trigger_origin_of_mem_childNodes (NodeWithAddress.mem_childNodes_of_mem_childNodes c_mem)
+        rw [NodeWithAddress.root_subderivation'] at this
+        apply FactSet.terms_subset_of_subset this.left
+        rw [List.mem_map] at t_mem
+        rcases t_mem with ⟨v, v_mem, t_mem⟩
+        rw [FactSet.mem_terms_toSet, PreTrigger.mem_terms_mapped_body_iff]
+        apply Or.inr
+        exists v; simp only [t_mem, and_true]
+        apply Rule.frontier_subset_vars_body; rw [Rule.mem_frontier_iff_mem_frontier_for_head]; exact ⟨_, v_mem⟩
+
+/-- If a functional term occurs in the chase, then the trigger that introduces this term must have been used in the chase, unless the term already occurs in the initial fact set. -/
+theorem trigger_introducing_functional_term_occurs_in_chase
+    {td : TreeDerivation obs rules}
+    (node : NodeWithAddress td)
+    {t : GroundTerm sig}
+    (t_mem_node : t ∈ node.node.facts.terms)
+    {trg : RTrigger obs rules}
+    {disj_idx : Nat}
+    {lt : disj_idx < trg.val.rule.head.length}
+    (t_mem_trg : t ∈ trg.val.fresh_terms_for_head_disjunct disj_idx lt) :
+    t ∈ td.root.facts.terms ∨ ∃ node2, node2 ≼ node ∧ ∃ orig ∈ node2.node.origin, orig.fst.equiv trg ∧ orig.snd.val = disj_idx := by
+  cases functional_term_originates_from_some_trigger node (by
+    cases eq : t with
+    | const _ =>
+      rw [eq] at t_mem_trg
+      simp [PreTrigger.fresh_terms_for_head_disjunct, PreTrigger.functional_term_for_var, GroundTerm.func, GroundTerm.const] at t_mem_trg
+    | func func ts arity_ok => exists func, ts, arity_ok
+  ) t_mem_node with
+  | inl t_mem => apply Or.inl; exact t_mem
+  | inr t_mem =>
+    apply Or.inr
+    rcases t_mem with ⟨node2, prec, origin, origin_eq, t_mem⟩
+    exists node2; simp only [prec, true_and]
+    exists origin; simp only [origin_eq, true_and]
+    exact RTrigger.equiv_of_term_mem_fresh_terms_for_head_disjunct t_mem t_mem_trg
+
+/-- If a functional term occurs in the chase, then the result of the trigger that introduces this term is contained in the current node, unless the functional term already occurs in the initial fact set. -/
+theorem result_of_trigger_introducing_functional_term_occurs_in_chase
+    {td : TreeDerivation obs rules}
+    (node : NodeWithAddress td)
+    {t : GroundTerm sig}
+    (t_mem_node : t ∈ node.node.facts.terms)
+    {trg : RTrigger obs rules}
+    {disj_idx : Nat}
+    {lt : disj_idx < trg.val.rule.head.length}
+    (t_mem_trg : t ∈ trg.val.fresh_terms_for_head_disjunct disj_idx lt) :
+    t ∈ td.root.facts.terms ∨ (trg.val.mapped_head[disj_idx]'(by rw [PreTrigger.length_mapped_head]; exact lt)).toSet ⊆ node.node.facts := by
+  cases trigger_introducing_functional_term_occurs_in_chase node t_mem_node t_mem_trg with
+  | inl t_mem => apply Or.inl; exact t_mem
+  | inr t_mem =>
+    apply Or.inr
+    rcases t_mem with ⟨node2, prec, origin, origin_eq, equiv, index_eq⟩
+    apply Set.subset_trans _ (td.facts_node_subset_of_prec prec)
+    simp only [← PreTrigger.result_eq_of_equiv equiv, ← index_eq]
+    exact node2.node.facts_contain_origin_result _ origin_eq
+
+end TermsInChase
 
 end TreeDerivation
 
