ExistentialRules/ChaseSequence/ChaseBranch.lean
@@ -1,7 +1,20 @@
 import ExistentialRules.ChaseSequence.ChaseDerivation
 
+/-!
+# Chase Branch
+
+A `ChaseBranch` is a special kind of `ChaseDerivation` which is defined for a `KnowledgeBase`
+and enforces the head of the `ChaseDerivation` to be the database from the `KnowledgeBase`.
+This is arguably the most common way for defining chase sequences/derivations in the literature.
+We call this branch here, since we consider rules with disjunctions that would actually create a chase tree (see `TreeDerivation` and `ChaseTree`)
+and intuitively the `ChaseBranch` is a branch in such a tree. However, it can be defined outside the tree, which is what we do here (and mostly did for the `ChaseDerivation already).
+
+Compared to the `ChaseDerivation` some new theorems can be shown or some existing ones strengthened. For example, we know now that functional terms can never occur in a database so every functional term must originate as a fresh term from some trigger that is used in the chase.
+-/
+
 variable {sig : Signature} [DecidableEq sig.P] [DecidableEq sig.C] [DecidableEq sig.V]
 
+/-- The `ChaseBranch` merely extends the `ChaseDerivation` with the condition that the head is the database from the knowledge base. -/
 structure ChaseBranch (obs : ObsoletenessCondition sig) (kb : KnowledgeBase sig) extends ChaseDerivation obs kb.rules where
   database_first : branch.head = some {
     facts := kb.db.toFactSet,
@@ -11,83 +24,91 @@ structure ChaseBranch (obs : ObsoletenessCondition sig) (kb : KnowledgeBase sig)
 
 namespace ChaseBranch
 
-  variable {obs : ObsoletenessCondition sig} {kb : KnowledgeBase sig}
+variable {obs : ObsoletenessCondition sig} {kb : KnowledgeBase sig}
 
-  theorem database_first' {cb : ChaseBranch obs kb} : cb.head = {
-    facts := kb.db.toFactSet,
-    origin := none,
-    facts_contain_origin_result := by simp
-  } := by simp only [ChaseDerivation.head, cb.database_first, Option.get_some]
+/-- We restate the `database_first` condition in terms of the `ChaseDerivation` vocabulary. -/
+theorem database_first' {cb : ChaseBranch obs kb} : cb.head = {
+  facts := kb.db.toFactSet,
+  origin := none,
+  facts_contain_origin_result := by simp
+} := by simp only [ChaseDerivation.head, cb.database_first, Option.get_some]
 
-  theorem facts_finite_of_mem {cb : ChaseBranch obs kb} (node : cb.Node) : node.val.facts.finite := by
-    induction node using ChaseDerivation.mem_rec with
-    | head => simp only [database_first']; exact kb.db.toFactSet.property.left
-    | step cd2 suffix ih next next_mem =>
-      rw [cd2.facts_next next_mem]
-      apply Set.union_finite_of_both_finite ih
-      apply List.finite_toSet
+/-- Opposed to a `ChaseDerivation`, we know that each node in a `ChaseBranch` has a finite set of facts. This is because the database is finite and each trigger only adds finitely many new facts. -/
+theorem facts_finite_of_mem {cb : ChaseBranch obs kb} (node : cb.Node) : node.val.facts.finite := by
+  induction node using ChaseDerivation.mem_rec with
+  | head => simp only [database_first']; exact kb.db.toFactSet.property.left
+  | step cd2 suffix ih next next_mem =>
+    rw [cd2.facts_next next_mem]
+    apply Set.union_finite_of_both_finite ih
+    apply List.finite_toSet
 
-  theorem func_term_not_mem_head {cb : ChaseBranch obs kb} {t : GroundTerm sig} (t_is_func : ∃ func ts arity_ok, t = GroundTerm.func func ts arity_ok) : ¬ t ∈ cb.head.facts.terms := by
-    intro t_mem
-    simp only [database_first'] at t_mem
-    rcases t_mem with ⟨f, f_mem, t_mem⟩
-    rcases kb.db.toFactSet.property.right f f_mem t t_mem with ⟨c, t_eq⟩
-    rcases t_is_func with ⟨_, _, _, t_eq'⟩
-    rw [t_eq'] at t_eq
-    simp [GroundTerm.const, GroundTerm.func] at t_eq
+/-- The head of the `ChaseBranch` does not contain any function terms. -/
+theorem func_term_not_mem_head {cb : ChaseBranch obs kb} {t : GroundTerm sig} (t_is_func : ∃ func ts arity_ok, t = GroundTerm.func func ts arity_ok) : ¬ t ∈ cb.head.facts.terms := by
+  intro t_mem
+  simp only [database_first'] at t_mem
+  rcases t_mem with ⟨f, f_mem, t_mem⟩
+  rcases kb.db.toFactSet.property.right f f_mem t t_mem with ⟨c, t_eq⟩
+  rcases t_is_func with ⟨_, _, _, t_eq'⟩
+  rw [t_eq'] at t_eq
+  simp [GroundTerm.const, GroundTerm.func] at t_eq
 
-  theorem constants_node_subset_constants_db_union_constants_rules {cb : ChaseBranch obs kb} {node : cb.Node} :
-      node.val.facts.constants ⊆ (kb.db.constants.val ∪ kb.rules.head_constants) := by
-    have := cb.constants_node_subset_constants_fs_union_constants_rules node.property
-    simp only [cb.database_first', Database.toFactSet_constants_same] at this
-    exact this
+/-- The result of a `ChaseBranch` not only models the rule set but the whole `KnowledgeBase`. -/
+theorem result_models_kb {cb : ChaseBranch obs kb} : cb.result.modelsKb kb := by
+  constructor
+  . intro f h
+    apply cb.facts_node_subset_result cb.head
+    . apply cb.head_mem
+    . rw [database_first']; exact h
+  . exact cb.result_models_rules
 
-  theorem result_models_kb {cb : ChaseBranch obs kb} : cb.result.modelsKb kb := by
-    constructor
-    . intro f h
-      apply cb.facts_node_subset_result cb.head
-      . apply cb.head_mem
-      . rw [database_first']; exact h
-    . exact cb.result_models_rules
+/-- Constants in the chase must be in the database or in some rule. -/
+theorem constants_node_subset_constants_db_union_constants_rules {cb : ChaseBranch obs kb} {node : cb.Node} :
+    node.val.facts.constants ⊆ (kb.db.constants.val ∪ kb.rules.head_constants) := by
+  have := cb.constants_node_subset_constants_fs_union_constants_rules node.property
+  simp only [cb.database_first', Database.toFactSet_constants_same] at this
+  exact this
 
-  theorem functional_term_originates_from_some_trigger
-      {cb : ChaseBranch obs kb}
-      (node : cb.Node)
-      {t : GroundTerm sig}
-      (t_is_func : ∃ func ts arity_ok, t = GroundTerm.func func ts arity_ok)
-      (t_mem : t ∈ node.val.facts.terms) :
-      ∃ node2, node2 ≼ node ∧ ∃ orig ∈ node2.val.origin, t ∈ orig.fst.val.fresh_terms_for_head_disjunct orig.snd.val (by rw [← PreTrigger.length_mapped_head]; exact orig.snd.isLt) := by
-    cases ChaseDerivation.functional_term_originates_from_some_trigger node t_is_func t_mem with
-    | inl t_mem => apply False.elim; exact cb.func_term_not_mem_head t_is_func t_mem
-    | inr t_mem => exact t_mem
+/-- Each functional term in the chase originates as a fresh term from a trigger. -/
+theorem functional_term_originates_from_some_trigger
+    {cb : ChaseBranch obs kb}
+    (node : cb.Node)
+    {t : GroundTerm sig}
+    (t_is_func : ∃ func ts arity_ok, t = GroundTerm.func func ts arity_ok)
+    (t_mem : t ∈ node.val.facts.terms) :
+    ∃ node2, node2 ≼ node ∧ ∃ orig ∈ node2.val.origin, t ∈ orig.fst.val.fresh_terms_for_head_disjunct orig.snd.val (by rw [← PreTrigger.length_mapped_head]; exact orig.snd.isLt) := by
+  cases ChaseDerivation.functional_term_originates_from_some_trigger node t_is_func t_mem with
+  | inl t_mem => apply False.elim; exact cb.func_term_not_mem_head t_is_func t_mem
+  | inr t_mem => exact t_mem
 
-  theorem trigger_introducing_functional_term_occurs_in_chase
-      {cb : ChaseBranch obs kb}
-      (node : cb.Node)
-      {t : GroundTerm sig}
-      (t_mem_node : t ∈ node.val.facts.terms)
-      {trg : RTrigger obs kb.rules}
-      {disj_idx : Nat}
-      {lt : disj_idx < trg.val.rule.head.length}
-      (t_mem_trg : t ∈ trg.val.fresh_terms_for_head_disjunct disj_idx lt) :
-      ∃ node2, node2 ≼ node ∧ ∃ orig ∈ node2.val.origin, orig.fst.equiv trg ∧ orig.snd.val = disj_idx := by
-    cases ChaseDerivation.trigger_introducing_functional_term_occurs_in_chase node t_mem_node t_mem_trg with
-    | inl t_mem => apply False.elim; exact cb.func_term_not_mem_head (PreTrigger.term_functional_of_mem_fresh_terms _ t_mem_trg) t_mem
-    | inr t_mem => exact t_mem
+/-- If a functional term occurs in the chase, then the trigger that introduces this term must have been used in the chase. -/
+theorem trigger_introducing_functional_term_occurs_in_chase
+    {cb : ChaseBranch obs kb}
+    (node : cb.Node)
+    {t : GroundTerm sig}
+    (t_mem_node : t ∈ node.val.facts.terms)
+    {trg : RTrigger obs kb.rules}
+    {disj_idx : Nat}
+    {lt : disj_idx < trg.val.rule.head.length}
+    (t_mem_trg : t ∈ trg.val.fresh_terms_for_head_disjunct disj_idx lt) :
+    ∃ node2, node2 ≼ node ∧ ∃ orig ∈ node2.val.origin, orig.fst.equiv trg ∧ orig.snd.val = disj_idx := by
+  cases ChaseDerivation.trigger_introducing_functional_term_occurs_in_chase node t_mem_node t_mem_trg with
+  | inl t_mem => apply False.elim; exact cb.func_term_not_mem_head (PreTrigger.term_functional_of_mem_fresh_terms _ t_mem_trg) t_mem
+  | inr t_mem => exact t_mem
 
-  theorem result_of_trigger_introducing_functional_term_occurs_in_chase
-      {cb : ChaseBranch obs kb}
-      (node : cb.Node)
-      {t : GroundTerm sig}
-      (t_mem_node : t ∈ node.val.facts.terms)
-      {trg : RTrigger obs kb.rules}
-      {disj_idx : Nat}
-      {lt : disj_idx < trg.val.rule.head.length}
-      (t_mem_trg : t ∈ trg.val.fresh_terms_for_head_disjunct disj_idx lt) :
-      (trg.val.mapped_head[disj_idx]'(by rw [PreTrigger.length_mapped_head]; exact lt)).toSet ⊆ node.val.facts := by
-    cases ChaseDerivation.result_of_trigger_introducing_functional_term_occurs_in_chase node t_mem_node t_mem_trg with
-    | inl t_mem => apply False.elim; exact cb.func_term_not_mem_head (PreTrigger.term_functional_of_mem_fresh_terms _ t_mem_trg) t_mem
-    | inr t_mem => exact t_mem
+/-- If a functional term occurs in the chase, then the result of the trigger that introduces this term is contained in the current node. -/
+theorem result_of_trigger_introducing_functional_term_occurs_in_chase
+    {cb : ChaseBranch obs kb}
+    (node : cb.Node)
+    {t : GroundTerm sig}
+    (t_mem_node : t ∈ node.val.facts.terms)
+    {trg : RTrigger obs kb.rules}
+    {disj_idx : Nat}
+    {lt : disj_idx < trg.val.rule.head.length}
+    (t_mem_trg : t ∈ trg.val.fresh_terms_for_head_disjunct disj_idx lt) :
+    (trg.val.mapped_head[disj_idx]'(by rw [PreTrigger.length_mapped_head]; exact lt)).toSet ⊆ node.val.facts := by
+  cases ChaseDerivation.result_of_trigger_introducing_functional_term_occurs_in_chase node t_mem_node t_mem_trg with
+  | inl t_mem => apply False.elim; exact cb.func_term_not_mem_head (PreTrigger.term_functional_of_mem_fresh_terms _ t_mem_trg) t_mem
+  | inr t_mem => exact t_mem
 
 end ChaseBranch
 
