ExistentialRules/ChaseSequence/ChaseNode.lean
@@ -2,6 +2,15 @@ import ExistentialRules.Triggers.RTrigger
 
 variable {sig : Signature} [DecidableEq sig.P] [DecidableEq sig.C] [DecidableEq sig.V]
 
+/-!
+# Chase Node
+
+The chase is a pretty simple procedure. From an initial fact set, it creates a new fact set by applying a trigger and it continues to do this until all triggers are obsolete.
+In this process, we obtain a (potentially infinite) sequence of fact sets.
+It can be very useful to also keep track of the associated triggers and this is why we capture both the fact set and used trigger of individual chase steps in a `ChaseNode`.
+-/
+
+/-- A `ChaseNode` corresponds to a chase step. It must contain a `FactSet` and optionally an `RTrigger` and a head disjunct index indicating that the current `ChaseNode` was obtained by applying the specified trigger and picking the indicated head disjunct. It is optional since the initial fact set does not result from a trigger but on all following nodes, this value will be set (and we will prove that it is). For convenience, the chase node also directly includes a proof that the result of its origin is indeed contained in its fact set. -/
 structure ChaseNode (obs : ObsoletenessCondition sig) (rules : RuleSet sig) where
   facts : FactSet sig
   -- the origin is none only for the database
@@ -10,10 +19,11 @@ structure ChaseNode (obs : ObsoletenessCondition sig) (rules : RuleSet sig) wher
 
 namespace ChaseNode
 
-  def origin_result {obs : ObsoletenessCondition sig} (node : ChaseNode obs rules) (isSome : node.origin.isSome) :
-      List (Fact sig) :=
-    let origin := node.origin.get isSome
-    origin.fst.val.mapped_head[origin.snd.val]
+/-- The `origin_result` denotes the facts that have been introduced for the chase node. That is, the mapped head index for the trigger stored in the origin field of the `ChaseNode`. -/
+def origin_result {obs : ObsoletenessCondition sig} (node : ChaseNode obs rules) (isSome : node.origin.isSome) :
+    List (Fact sig) :=
+  let origin := node.origin.get isSome
+  origin.fst.val.mapped_head[origin.snd.val]
 
 end ChaseNode
 
