ExistentialRules/ChaseSequence/ChaseTree.lean
@@ -1,8 +1,20 @@
 import ExistentialRules.ChaseSequence.ChaseBranch
 import ExistentialRules.ChaseSequence.TreeDerivation
 
+/-!
+# Chase Tree
+
+A `ChaseTree` is a special kind of `TreeDerivation` which is defined for a `KnowledgeBase`
+and enforces the root of the `TreeDerivation` to be the database from the `KnowledgeBase`.
+
+Compared to the `TreeDerivation` some new theorems can be shown or some existing ones strengthened. For example, we know now that functional terms can never occur in a database so every functional term must originate as a fresh term from some trigger that is used in the chase.
+
+The `ChaseTree` is to the `TreeDerivation` what the `ChaseBranch` is to the `ChaseDerivation`.
+-/
+
 variable {sig : Signature} [DecidableEq sig.P] [DecidableEq sig.C] [DecidableEq sig.V]
 
+/-- The `ChaseTree` merely extends the `TreeDerivation` with the condition that the root is the database from the knowledge base. -/
 structure ChaseTree (obs : ObsoletenessCondition sig) (kb : KnowledgeBase sig) extends TreeDerivation obs kb.rules where
   database_first : tree.root = some {
     facts := kb.db.toFactSet
@@ -12,97 +24,106 @@ structure ChaseTree (obs : ObsoletenessCondition sig) (kb : KnowledgeBase sig) e
 
 namespace ChaseTree
 
-  variable {obs : ObsoletenessCondition sig} {kb : KnowledgeBase sig}
+variable {obs : ObsoletenessCondition sig} {kb : KnowledgeBase sig}
 
-  instance : Membership (ChaseNode obs kb.rules) (ChaseTree obs kb) where
-    mem td node := node ∈ td.tree
+instance : Membership (ChaseNode obs kb.rules) (ChaseTree obs kb) where
+  mem td node := node ∈ td.tree
 
-  def chaseBranch_for_branch {ct : ChaseTree obs kb} {branch : ChaseDerivation obs kb.rules} (branch_mem : branch ∈ ct.branches) : ChaseBranch obs kb := {
-    branch := branch.branch
-    isSome_head := branch.isSome_head
-    triggers_exist := branch.triggers_exist
-    fairness := branch.fairness
-    database_first := by rw [← ct.database_first]; unfold TreeDerivation.branches at branch_mem; rw [FiniteDegreeTree.branches_eq] at branch_mem; rw [branch_mem.left]
-  }
+/-- We can convert `ChaseDerivation`s that are branches in the `ChaseTree` to `ChaseBranch`es. -/
+def chaseBranch_for_branch {ct : ChaseTree obs kb} {branch : ChaseDerivation obs kb.rules} (branch_mem : branch ∈ ct.branches) : ChaseBranch obs kb := {
+  branch := branch.branch
+  isSome_head := branch.isSome_head
+  triggers_exist := branch.triggers_exist
+  fairness := branch.fairness
+  database_first := by rw [← ct.database_first]; unfold TreeDerivation.branches at branch_mem; rw [FiniteDegreeTree.branches_eq] at branch_mem; rw [branch_mem.left]
+}
 
-  theorem database_first' {ct : ChaseTree obs kb} : ct.root = {
-    facts := kb.db.toFactSet,
-    origin := none,
-    facts_contain_origin_result := by simp
-  } := by simp only [TreeDerivation.root, ct.database_first, Option.get_some]
+/-- We restate the `database_first` condition in terms of the `TreeDerivation` vocabulary. -/
+theorem database_first' {ct : ChaseTree obs kb} : ct.root = {
+  facts := kb.db.toFactSet,
+  origin := none,
+  facts_contain_origin_result := by simp
+} := by simp only [TreeDerivation.root, ct.database_first, Option.get_some]
 
-  theorem facts_finite_of_mem {ct : ChaseTree obs kb} {node : ChaseNode obs kb.rules} (node_mem : node ∈ ct) : node.facts.finite := by
-    rcases node_mem with ⟨addr, node_mem⟩
-    let node' : ct.NodeWithAddress := {node := node, address := addr, eq := node_mem}
-    show node'.node.facts.finite
-    induction node' using TreeDerivation.mem_rec_address with
-    | root => simp only [TreeDerivation.root_NodeWithAddress, database_first']; exact kb.db.toFactSet.property.left
-    | step new_root ih c c_mem =>
-      simp only [TreeDerivation.NodeWithAddress.cast_for_new_root_node]
-      rw [TreeDerivation.facts_childNodes (TreeDerivation.mem_childNodes_of_mem_childNodes_as_NodesWithAddress c_mem)]
-      rw [TreeDerivation.root_subderivation_for_NodeWithAddress]
-      apply Set.union_finite_of_both_finite ih
-      apply List.finite_toSet
+/-- Opposed to a `TreeDerivation`, we know that each node in a `ChaseBranch` has a finite set of facts. This is because the database is finite and each trigger only adds finitely many new facts. -/
+theorem facts_finite_of_mem {ct : ChaseTree obs kb} {node : ChaseNode obs kb.rules} (node_mem : node ∈ ct) : node.facts.finite := by
+  rcases node_mem with ⟨addr, node_mem⟩
+  let node' : ct.NodeWithAddress := {node := node, address := addr, eq := node_mem}
+  show node'.node.facts.finite
+  induction node' using TreeDerivation.mem_rec_address with
+  | root => simp only [TreeDerivation.NodeWithAddress.root, database_first']; exact kb.db.toFactSet.property.left
+  | step new_root ih c c_mem =>
+    simp only [TreeDerivation.NodeWithAddress.cast_for_new_root_node]
+    rw [TreeDerivation.facts_childNodes (TreeDerivation.NodeWithAddress.mem_childNodes_of_mem_childNodes c_mem)]
+    rw [TreeDerivation.NodeWithAddress.root_subderivation']
+    apply Set.union_finite_of_both_finite ih
+    apply List.finite_toSet
 
-  theorem func_term_not_mem_head {ct : ChaseTree obs kb} {t : GroundTerm sig} (t_is_func : ∃ func ts arity_ok, t = GroundTerm.func func ts arity_ok) : ¬ t ∈ ct.root.facts.terms := by
-    intro t_mem
-    simp only [database_first'] at t_mem
-    rcases t_mem with ⟨f, f_mem, t_mem⟩
-    rcases kb.db.toFactSet.property.right f f_mem t t_mem with ⟨c, t_eq⟩
-    rcases t_is_func with ⟨_, _, _, t_eq'⟩
-    rw [t_eq'] at t_eq
-    simp [GroundTerm.const, GroundTerm.func] at t_eq
+/-- The root of the `ChaseTree` does not contain any function terms. -/
+theorem func_term_not_mem_root {ct : ChaseTree obs kb} {t : GroundTerm sig} (t_is_func : ∃ func ts arity_ok, t = GroundTerm.func func ts arity_ok) : ¬ t ∈ ct.root.facts.terms := by
+  intro t_mem
+  simp only [database_first'] at t_mem
+  rcases t_mem with ⟨f, f_mem, t_mem⟩
+  rcases kb.db.toFactSet.property.right f f_mem t t_mem with ⟨c, t_eq⟩
+  rcases t_is_func with ⟨_, _, _, t_eq'⟩
+  rw [t_eq'] at t_eq
+  simp [GroundTerm.const, GroundTerm.func] at t_eq
 
-  theorem constants_node_subset_constants_db_union_constants_rules {ct : ChaseTree obs kb} {node : ChaseNode obs kb.rules} (node_mem : node ∈ ct) :
-      node.facts.constants ⊆ (kb.db.constants.val ∪ kb.rules.head_constants) := by
-    have := ct.constants_node_subset_constants_fs_union_constants_rules node_mem
-    simp only [ct.database_first', Database.toFactSet_constants_same] at this
-    exact this
+/-- Each element of the result of a `ChaseTree` not only models the rule set but the whole `KnowledgeBase`. -/
+theorem result_models_kb {ct : ChaseTree obs kb} : ∀ fs ∈ ct.result, fs.modelsKb kb := by
+  rintro fs ⟨branch, branch_mem, fs_mem⟩
+  let cb := ct.chaseBranch_for_branch branch_mem
+  have : branch.result = cb.result := by rfl
+  rw [fs_mem, this]
+  exact cb.result_models_kb
 
-  theorem result_models_kb {ct : ChaseTree obs kb} : ∀ fs ∈ ct.result, fs.modelsKb kb := by
-    rintro fs ⟨branch, branch_mem, fs_mem⟩
-    let cb := ct.chaseBranch_for_branch branch_mem
-    have : branch.result = cb.result := by rfl
-    rw [← fs_mem, this]
-    exact cb.result_models_kb
+/-- Constants in the chase must be in the database or in some rule. -/
+theorem constants_node_subset_constants_db_union_constants_rules {ct : ChaseTree obs kb} {node : ChaseNode obs kb.rules} (node_mem : node ∈ ct) :
+    node.facts.constants ⊆ (kb.db.constants.val ∪ kb.rules.head_constants) := by
+  have := ct.constants_node_subset_constants_fs_union_constants_rules node_mem
+  simp only [ct.database_first', Database.toFactSet_constants_same] at this
+  exact this
 
-  theorem functional_term_originates_from_some_trigger
-      {ct : ChaseTree obs kb}
-      (node : ct.NodeWithAddress)
-      {t : GroundTerm sig}
-      (t_is_func : ∃ func ts arity_ok, t = GroundTerm.func func ts arity_ok)
-      (t_mem : t ∈ node.node.facts.terms) :
-      ∃ node2, node2 ≼ node ∧ ∃ orig ∈ node2.node.origin, t ∈ orig.fst.val.fresh_terms_for_head_disjunct orig.snd.val (by rw [← PreTrigger.length_mapped_head]; exact orig.snd.isLt) := by
-    cases TreeDerivation.functional_term_originates_from_some_trigger node t_is_func t_mem with
-    | inl t_mem => apply False.elim; exact ct.func_term_not_mem_head t_is_func t_mem
-    | inr t_mem => exact t_mem
+/-- Each functional term in the chase originates as a fresh term from a trigger. -/
+theorem functional_term_originates_from_some_trigger
+    {ct : ChaseTree obs kb}
+    (node : ct.NodeWithAddress)
+    {t : GroundTerm sig}
+    (t_is_func : ∃ func ts arity_ok, t = GroundTerm.func func ts arity_ok)
+    (t_mem : t ∈ node.node.facts.terms) :
+    ∃ node2, node2 ≼ node ∧ ∃ orig ∈ node2.node.origin, t ∈ orig.fst.val.fresh_terms_for_head_disjunct orig.snd.val (by rw [← PreTrigger.length_mapped_head]; exact orig.snd.isLt) := by
+  cases TreeDerivation.functional_term_originates_from_some_trigger node t_is_func t_mem with
+  | inl t_mem => apply False.elim; exact ct.func_term_not_mem_root t_is_func t_mem
+  | inr t_mem => exact t_mem
 
-  theorem trigger_introducing_functional_term_occurs_in_chase
-      {ct : ChaseTree obs kb}
-      (node : ct.NodeWithAddress)
-      {t : GroundTerm sig}
-      (t_mem_node : t ∈ node.node.facts.terms)
-      {trg : RTrigger obs kb.rules}
-      {disj_idx : Nat}
-      {lt : disj_idx < trg.val.rule.head.length}
-      (t_mem_trg : t ∈ trg.val.fresh_terms_for_head_disjunct disj_idx lt) :
-      ∃ node2, node2 ≼ node ∧ ∃ orig ∈ node2.node.origin, orig.fst.equiv trg ∧ orig.snd.val = disj_idx := by
-    cases TreeDerivation.trigger_introducing_functional_term_occurs_in_chase node t_mem_node t_mem_trg with
-    | inl t_mem => apply False.elim; exact ct.func_term_not_mem_head (PreTrigger.term_functional_of_mem_fresh_terms _ t_mem_trg) t_mem
-    | inr t_mem => exact t_mem
+/-- If a functional term occurs in the chase, then the trigger that introduces this term must have been used in the chase. -/
+theorem trigger_introducing_functional_term_occurs_in_chase
+    {ct : ChaseTree obs kb}
+    (node : ct.NodeWithAddress)
+    {t : GroundTerm sig}
+    (t_mem_node : t ∈ node.node.facts.terms)
+    {trg : RTrigger obs kb.rules}
+    {disj_idx : Nat}
+    {lt : disj_idx < trg.val.rule.head.length}
+    (t_mem_trg : t ∈ trg.val.fresh_terms_for_head_disjunct disj_idx lt) :
+    ∃ node2, node2 ≼ node ∧ ∃ orig ∈ node2.node.origin, orig.fst.equiv trg ∧ orig.snd.val = disj_idx := by
+  cases TreeDerivation.trigger_introducing_functional_term_occurs_in_chase node t_mem_node t_mem_trg with
+  | inl t_mem => apply False.elim; exact ct.func_term_not_mem_root (PreTrigger.term_functional_of_mem_fresh_terms _ t_mem_trg) t_mem
+  | inr t_mem => exact t_mem
 
-  theorem result_of_trigger_introducing_functional_term_occurs_in_chase
-      {ct : ChaseTree obs kb}
-      (node : ct.NodeWithAddress)
-      {t : GroundTerm sig}
-      (t_mem_node : t ∈ node.node.facts.terms)
-      {trg : RTrigger obs kb.rules}
-      {disj_idx : Nat}
-      {lt : disj_idx < trg.val.rule.head.length}
-      (t_mem_trg : t ∈ trg.val.fresh_terms_for_head_disjunct disj_idx lt) :
-      (trg.val.mapped_head[disj_idx]'(by rw [PreTrigger.length_mapped_head]; exact lt)).toSet ⊆ node.node.facts := by
-    cases TreeDerivation.result_of_trigger_introducing_functional_term_occurs_in_chase node t_mem_node t_mem_trg with
-    | inl t_mem => apply False.elim; exact ct.func_term_not_mem_head (PreTrigger.term_functional_of_mem_fresh_terms _ t_mem_trg) t_mem
-    | inr t_mem => exact t_mem
+/-- If a functional term occurs in the chase, then the result of the trigger that introduces this term is contained in the current node. -/
+theorem result_of_trigger_introducing_functional_term_occurs_in_chase
+    {ct : ChaseTree obs kb}
+    (node : ct.NodeWithAddress)
+    {t : GroundTerm sig}
+    (t_mem_node : t ∈ node.node.facts.terms)
+    {trg : RTrigger obs kb.rules}
+    {disj_idx : Nat}
+    {lt : disj_idx < trg.val.rule.head.length}
+    (t_mem_trg : t ∈ trg.val.fresh_terms_for_head_disjunct disj_idx lt) :
+    (trg.val.mapped_head[disj_idx]'(by rw [PreTrigger.length_mapped_head]; exact lt)).toSet ⊆ node.node.facts := by
+  cases TreeDerivation.result_of_trigger_introducing_functional_term_occurs_in_chase node t_mem_node t_mem_trg with
+  | inl t_mem => apply False.elim; exact ct.func_term_not_mem_root (PreTrigger.term_functional_of_mem_fresh_terms _ t_mem_trg) t_mem
+  | inr t_mem => exact t_mem
 
 end ChaseTree
